<?xml version="1.0"?>
<rdf:RDF xmlns="http://purl.org/htp#"
     xml:base="http://purl.org/htp"
     xmlns:dc="http://purl.org/dc/elements/1.1/"
     xmlns:htp="http://purl.org/htp#"
     xmlns:iao="http://purl.obolibrary.org/obo/iao"
     xmlns:obo="http://purl.obolibrary.org/obo/"
     xmlns:owl="http://www.w3.org/2002/07/owl#"
     xmlns:rdf="http://www.w3.org/1999/02/22-rdf-syntax-ns#"
     xmlns:xml="http://www.w3.org/XML/1998/namespace"
     xmlns:xsd="http://www.w3.org/2001/XMLSchema#"
     xmlns:foaf="http://xmlns.com/foaf/0.1/"
     xmlns:rdfs="http://www.w3.org/2000/01/rdf-schema#"
     xmlns:skos="http://www.w3.org/2004/02/skos/core#"
     xmlns:dcterms="http://purl.org/dc/terms/">
    <owl:Ontology rdf:about="http://purl.org/htp">
        <obo:iaoIAO_0000115 rdf:resource="http://purl.obolibrary.org/obo/iao.owl"/>
        <dcterms:contributor>Prof. Dr. Nils Opel</dcterms:contributor>
        <dcterms:creator>
            <rdf:Description>
                <rdf:type rdf:resource="http://xmlns.com/foaf/0.1/Person"/>
                <foaf:mbox rdf:resource="mailto:rogerio.blitz@med.uni-jena.de"/>
                <foaf:name>Dr. Rogério Blitz</foaf:name>
            </rdf:Description>
        </dcterms:creator>
        <dcterms:date>2024-08-30</dcterms:date>
        <dcterms:hasVersion rdf:resource="http://purl.org/dc/terms/1.1"/>
        <dcterms:isVersionOf rdf:resource="http://purl.org/dc/terms/1.1"/>
        <dcterms:issued rdf:resource="http://purl.org/dc/terms/1.1"/>
        <dcterms:issued>2024-08-18</dcterms:issued>
        <dcterms:license rdf:resource="https://creativecommons.org/licenses/by-nc-nd/4.0/"/>
        <dcterms:publisher>Dr. Rogério Blitz, Prof. Dr. Nils Opel</dcterms:publisher>
        <dcterms:rights>This work is licensed under a Creative Commons Attribution-NonCommercial-NoDerivs 4.0 International License.</dcterms:rights>
        <dcterms:rightsHolder>Dr. Rogério Blitz, Prof. Dr. Nils Opel</dcterms:rightsHolder>
        <dcterms:rightsHolder>Universitätsklinikum Jena</dcterms:rightsHolder>
        <rdfs:comment>Dynamic Ontology for Mental Health Classification representing various classes to structure mental health dimensions in the HiTOP model.</rdfs:comment>
        <rdfs:label>Dynamic Ontology for Mental Health Classification</rdfs:label>
        <rdfs:seeAlso rdf:resource="https://www.hitop-system.org/"/>
        <owl:versionInfo rdf:datatype="http://www.w3.org/2001/XMLSchema#decimal">1.7</owl:versionInfo>
        <skos:changeNote rdf:resource="https://www.w3.org/2009/08/skos-reference/skos.html"/>
    </owl:Ontology>
    


    <!-- 
    ///////////////////////////////////////////////////////////////////////////////////////
    //
    // Annotation properties
    //
    ///////////////////////////////////////////////////////////////////////////////////////
     -->

    


    <!-- http://purl.obolibrary.org/obo/iaoIAO_0000115 -->

    <owl:AnnotationProperty rdf:about="http://purl.obolibrary.org/obo/iaoIAO_0000115"/>
    


    <!-- http://purl.org/dc/terms/contributor -->

    <owl:AnnotationProperty rdf:about="http://purl.org/dc/terms/contributor"/>
    


    <!-- http://purl.org/dc/terms/creator -->

    <owl:AnnotationProperty rdf:about="http://purl.org/dc/terms/creator"/>
    


    <!-- http://purl.org/dc/terms/date -->

    <owl:AnnotationProperty rdf:about="http://purl.org/dc/terms/date"/>
    


    <!-- http://purl.org/dc/terms/hasVersion -->

    <owl:AnnotationProperty rdf:about="http://purl.org/dc/terms/hasVersion"/>
    


    <!-- http://purl.org/dc/terms/isVersionOf -->

    <owl:AnnotationProperty rdf:about="http://purl.org/dc/terms/isVersionOf"/>
    


    <!-- http://purl.org/dc/terms/issued -->

    <owl:AnnotationProperty rdf:about="http://purl.org/dc/terms/issued"/>
    


    <!-- http://purl.org/dc/terms/license -->

    <owl:AnnotationProperty rdf:about="http://purl.org/dc/terms/license"/>
    


    <!-- http://purl.org/dc/terms/publisher -->

    <owl:AnnotationProperty rdf:about="http://purl.org/dc/terms/publisher"/>
    


    <!-- http://purl.org/dc/terms/rights -->

    <owl:AnnotationProperty rdf:about="http://purl.org/dc/terms/rights"/>
    


    <!-- http://purl.org/dc/terms/rightsHolder -->

    <owl:AnnotationProperty rdf:about="http://purl.org/dc/terms/rightsHolder"/>
    


    <!-- http://www.w3.org/2004/02/skos/core#changeNote -->

    <owl:AnnotationProperty rdf:about="http://www.w3.org/2004/02/skos/core#changeNote"/>
    


    <!-- http://xmlns.com/foaf/0.1/mbox -->

    <owl:AnnotationProperty rdf:about="http://xmlns.com/foaf/0.1/mbox"/>
    


    <!-- http://xmlns.com/foaf/0.1/name -->

    <owl:AnnotationProperty rdf:about="http://xmlns.com/foaf/0.1/name"/>
    


    <!-- 
    ///////////////////////////////////////////////////////////////////////////////////////
    //
    // Object Properties
    //
    ///////////////////////////////////////////////////////////////////////////////////////
     -->

    


    <!-- http://purl.org/htp#hasFactor -->

    <owl:ObjectProperty rdf:about="http://purl.org/htp#hasFactor">
        <rdfs:domain rdf:resource="http://purl.org/htp#HiTOP-O001Ih"/>
        <rdfs:range rdf:resource="http://purl.org/htp#HiTOP-O001Ih"/>
        <rdfs:comment xml:lang="en">This property represents the highest level of the HiTOP taxonomy, associating entities with the psychopathology factor level, which encompasses broad constructs underlying mental health and psychological disorders.</rdfs:comment>
        <rdfs:label xml:lang="en">has Factor</rdfs:label>
        <skos:changeNote xml:lang="en">
            Indicates the possibility of extending or modifying the taxonomy at the factor level to incorporate new findings in the field of psychopathology. 
            This supports the evolution of the model to remain aligned with contemporary research.
        </skos:changeNote>
    </owl:ObjectProperty>
    


    <!-- http://purl.org/htp#hasLevel -->

    <owl:ObjectProperty rdf:about="http://purl.org/htp#hasLevel">
        <rdfs:domain rdf:resource="http://purl.org/htp#HiTOP-O001Ih"/>
        <rdfs:range rdf:resource="http://purl.org/htp#HiTOP-O001Ih"/>
        <rdfs:comment xml:lang="en">This property establishes a hierarchical relationship between entities, associating them with their respective level in the HiTOP taxonomy, such as psychopathology factors, superspectra, spectra, subfactors, or components.</rdfs:comment>
        <rdfs:label xml:lang="en">has Level</rdfs:label>
        <skos:changeNote xml:lang="en">
            Indicates the potential for future inclusion of additional levels or modification of existing ones to reflect new developments in the model.
            Supports flexibility in expanding or refining the taxonomy based on emerging research and evolving understanding of psychological constructs.
        </skos:changeNote>
    </owl:ObjectProperty>
    


    <!-- http://purl.org/htp#hasTier -->

    <owl:ObjectProperty rdf:about="http://purl.org/htp#hasTier">
        <rdfs:domain rdf:resource="http://purl.org/htp#HiTOP-O002sP"/>
        <rdfs:range rdf:resource="http://purl.org/htp#HiTOP-O002sP"/>
        <rdfs:comment xml:lang="en">This property establishes a horizontal relationship between entities within the same level of the HiTOP taxonomy, associating them with their respective tier, such as clusters, categories, or subcategories.</rdfs:comment>
        <rdfs:label xml:lang="en">has Tier</rdfs:label>
        <skos:changeNote xml:lang="en">
            Indicates the potential for future inclusion of additional tiers or modification of existing ones to reflect new developments within specific levels of the hierarchy. 
            Supports flexibility in expanding or refining the taxonomy based on emerging research and evolving understanding of horizontal relationships among psychological constructs.
        </skos:changeNote>
    </owl:ObjectProperty>
    


    <!-- http://purl.org/htp#partOfVersionHistory -->

    <owl:ObjectProperty rdf:about="http://purl.org/htp#partOfVersionHistory">
        <rdfs:subPropertyOf rdf:resource="http://purl.org/dc/terms/isPartOf"/>
        <rdfs:domain rdf:resource="http://purl.org/htp#hasVersionID"/>
        <rdfs:range rdf:resource="http://purl.org/htp#VersionHistory"/>
        <rdfs:comment xml:lang="en">Relates a version (e.g., Version_1_0) to the HiTOP Version History, linking a specific version to a version history entry.</rdfs:comment>
        <rdfs:label xml:lang="en">partOfVersionHistory</rdfs:label>
        <skos:changeNote xml:lang="en">
            This property supports the tracking of versioning and the documentation of changes over time in the HiTOP model, ensuring transparent version control.
        </skos:changeNote>
    </owl:ObjectProperty>
    


    <!-- 
    ///////////////////////////////////////////////////////////////////////////////////////
    //
    // Data properties
    //
    ///////////////////////////////////////////////////////////////////////////////////////
     -->

    


    <!-- http://purl.org/htp#hasVersionID -->

    <owl:DatatypeProperty rdf:about="http://purl.org/htp#hasVersionID">
        <rdfs:domain rdf:resource="http://purl.org/htp#HiTOP-C001qy"/>
        <rdfs:domain rdf:resource="http://purl.org/htp#HiTOP-C00217"/>
        <rdfs:domain rdf:resource="http://purl.org/htp#HiTOP-C0033z"/>
        <rdfs:domain rdf:resource="http://purl.org/htp#HiTOP-C00416"/>
        <rdfs:domain rdf:resource="http://purl.org/htp#HiTOP-C005Sv"/>
        <rdfs:domain rdf:resource="http://purl.org/htp#HiTOP-C006MD"/>
        <rdfs:domain rdf:resource="http://purl.org/htp#HiTOP-C00JTU"/>
        <rdfs:domain rdf:resource="http://purl.org/htp#HiTOP-C00KL0"/>
        <rdfs:domain rdf:resource="http://purl.org/htp#HiTOP-C00LqY"/>
        <rdfs:domain rdf:resource="http://purl.org/htp#HiTOP-C00Mpl"/>
        <rdfs:domain rdf:resource="http://purl.org/htp#HiTOP-C00N4I"/>
        <rdfs:domain rdf:resource="http://purl.org/htp#HiTOP-C00OuR"/>
        <rdfs:domain rdf:resource="http://purl.org/htp#HiTOP-C00Pjp"/>
        <rdfs:domain rdf:resource="http://purl.org/htp#HiTOP-C00Q1t"/>
        <rdfs:domain rdf:resource="http://purl.org/htp#HiTOP-C00RGy"/>
        <rdfs:domain rdf:resource="http://purl.org/htp#HiTOP-C00S9m"/>
        <rdfs:domain rdf:resource="http://purl.org/htp#HiTOP-C00TgL"/>
        <rdfs:domain rdf:resource="http://purl.org/htp#HiTOP-C00Urw"/>
        <rdfs:domain rdf:resource="http://purl.org/htp#HiTOP-C00VHv"/>
        <rdfs:domain rdf:resource="http://purl.org/htp#HiTOP-C00WJc"/>
        <rdfs:domain rdf:resource="http://purl.org/htp#HiTOP-C00XyI"/>
        <rdfs:domain rdf:resource="http://purl.org/htp#HiTOP-C00Y8j"/>
        <rdfs:domain rdf:resource="http://purl.org/htp#HiTOP-C00ZyP"/>
        <rdfs:domain rdf:resource="http://purl.org/htp#HiTOP-C00aMF"/>
        <rdfs:domain rdf:resource="http://purl.org/htp#HiTOP-C00bEx"/>
        <rdfs:domain rdf:resource="http://purl.org/htp#HiTOP-C00cSn"/>
        <rdfs:domain rdf:resource="http://purl.org/htp#HiTOP-C00dc1"/>
        <rdfs:domain rdf:resource="http://purl.org/htp#HiTOP-C00eL"/>
        <rdfs:domain rdf:resource="http://purl.org/htp#HiTOP-C00fKQ"/>
        <rdfs:domain rdf:resource="http://purl.org/htp#HiTOP-C00gvD"/>
        <rdfs:domain rdf:resource="http://purl.org/htp#HiTOP-C00hPJ"/>
        <rdfs:domain rdf:resource="http://purl.org/htp#HiTOP-C00iAh"/>
        <rdfs:domain rdf:resource="http://purl.org/htp#HiTOP-C00jw5"/>
        <rdfs:domain rdf:resource="http://purl.org/htp#HiTOP-C00kEN"/>
        <rdfs:domain rdf:resource="http://purl.org/htp#HiTOP-C00l5y"/>
        <rdfs:domain rdf:resource="http://purl.org/htp#HiTOP-C00mpe"/>
        <rdfs:domain rdf:resource="http://purl.org/htp#HiTOP-C00nyb"/>
        <rdfs:domain rdf:resource="http://purl.org/htp#HiTOP-C00oKM"/>
        <rdfs:domain rdf:resource="http://purl.org/htp#HiTOP-C00pnZ"/>
        <rdfs:domain rdf:resource="http://purl.org/htp#HiTOP-C00qSD"/>
        <rdfs:domain rdf:resource="http://purl.org/htp#HiTOP-C00rnS"/>
        <rdfs:domain rdf:resource="http://purl.org/htp#HiTOP-C00sWr"/>
        <rdfs:domain rdf:resource="http://purl.org/htp#HiTOP-C00tUQ"/>
        <rdfs:domain rdf:resource="http://purl.org/htp#HiTOP-C01DAb"/>
        <rdfs:domain rdf:resource="http://purl.org/htp#HiTOP-C01Elz"/>
        <rdfs:domain rdf:resource="http://purl.org/htp#HiTOP-C01FDy"/>
        <rdfs:domain rdf:resource="http://purl.org/htp#HiTOP-C01GEY"/>
        <rdfs:domain rdf:resource="http://purl.org/htp#HiTOP-C01HGq"/>
        <rdfs:domain rdf:resource="http://purl.org/htp#HiTOP-C01Ip4"/>
        <rdfs:domain rdf:resource="http://purl.org/htp#HiTOP-C01JH8"/>
        <rdfs:domain rdf:resource="http://purl.org/htp#HiTOP-C01KXo"/>
        <rdfs:domain rdf:resource="http://purl.org/htp#HiTOP-C01LSp"/>
        <rdfs:domain rdf:resource="http://purl.org/htp#HiTOP-C01MjB"/>
        <rdfs:domain rdf:resource="http://purl.org/htp#HiTOP-F001Hw"/>
        <rdfs:domain rdf:resource="http://purl.org/htp#HiTOP-P001Y2"/>
        <rdfs:domain rdf:resource="http://purl.org/htp#HiTOP-P002nf"/>
        <rdfs:domain rdf:resource="http://purl.org/htp#HiTOP-P003SL"/>
        <rdfs:domain rdf:resource="http://purl.org/htp#HiTOP-P004R1"/>
        <rdfs:domain rdf:resource="http://purl.org/htp#HiTOP-P005xY"/>
        <rdfs:domain rdf:resource="http://purl.org/htp#HiTOP-P006gM"/>
        <rdfs:domain rdf:resource="http://purl.org/htp#HiTOP-T007eM"/>
        <rdfs:domain rdf:resource="http://purl.org/htp#HiTOP-T008mD"/>
        <rdfs:domain rdf:resource="http://purl.org/htp#HiTOP-T0094I"/>
        <rdfs:domain rdf:resource="http://purl.org/htp#HiTOP-T00AZ"/>
        <rdfs:domain rdf:resource="http://purl.org/htp#HiTOP-T00BXK"/>
        <rdfs:domain rdf:resource="http://purl.org/htp#HiTOP-T00Cgy"/>
        <rdfs:domain rdf:resource="http://purl.org/htp#HiTOP-T00D42"/>
        <rdfs:domain rdf:resource="http://purl.org/htp#HiTOP-T00Eht"/>
        <rdfs:domain rdf:resource="http://purl.org/htp#HiTOP-T00Fe0"/>
        <rdfs:domain rdf:resource="http://purl.org/htp#HiTOP-T00G3d"/>
        <rdfs:domain rdf:resource="http://purl.org/htp#HiTOP-T00HCy"/>
        <rdfs:domain rdf:resource="http://purl.org/htp#HiTOP-T00IAT"/>
        <rdfs:domain rdf:resource="http://purl.org/htp#HiTOP-T00ua9"/>
        <rdfs:domain rdf:resource="http://purl.org/htp#HiTOP-T00vjR"/>
        <rdfs:domain rdf:resource="http://purl.org/htp#HiTOP-T00wk6"/>
        <rdfs:domain rdf:resource="http://purl.org/htp#HiTOP-T00xLn"/>
        <rdfs:domain rdf:resource="http://purl.org/htp#HiTOP-T00yfU"/>
        <rdfs:domain rdf:resource="http://purl.org/htp#HiTOP-T00zDk"/>
        <rdfs:domain rdf:resource="http://purl.org/htp#HiTOP-T010c6"/>
        <rdfs:domain rdf:resource="http://purl.org/htp#HiTOP-T011K6"/>
        <rdfs:domain rdf:resource="http://purl.org/htp#HiTOP-T012QL"/>
        <rdfs:domain rdf:resource="http://purl.org/htp#HiTOP-T013F1"/>
        <rdfs:domain rdf:resource="http://purl.org/htp#HiTOP-T014BA"/>
        <rdfs:domain rdf:resource="http://purl.org/htp#HiTOP-T015o8"/>
        <rdfs:domain rdf:resource="http://purl.org/htp#HiTOP-T016k0"/>
        <rdfs:domain rdf:resource="http://purl.org/htp#HiTOP-T0177S"/>
        <rdfs:domain rdf:resource="http://purl.org/htp#HiTOP-T018ir"/>
        <rdfs:domain rdf:resource="http://purl.org/htp#HiTOP-T019Cj"/>
        <rdfs:domain rdf:resource="http://purl.org/htp#HiTOP-T01A5i"/>
        <rdfs:domain rdf:resource="http://purl.org/htp#HiTOP-T01BfQ"/>
        <rdfs:domain rdf:resource="http://purl.org/htp#HiTOP-T01C1W"/>
        <rdfs:domain rdf:resource="http://purl.org/htp#HiTOP-T01Neb"/>
        <rdfs:domain rdf:resource="http://purl.org/htp#HiTOP-T01OY2"/>
        <rdfs:domain rdf:resource="http://purl.org/htp#HiTOP-T01PMW"/>
        <rdfs:domain rdf:resource="http://purl.org/htp#HiTOP-T01QNN"/>
        <rdfs:domain rdf:resource="http://purl.org/htp#HiTOP-T01RYG"/>
        <rdfs:domain rdf:resource="http://purl.org/htp#HiTOP-T01SYW"/>
        <rdfs:domain rdf:resource="http://purl.org/htp#HiTOP-T01T3u"/>
        <rdfs:domain rdf:resource="http://purl.org/htp#HiTOP-T01UGN"/>
        <rdfs:domain rdf:resource="http://purl.org/htp#HiTOP-T01VXq"/>
        <rdfs:domain rdf:resource="http://purl.org/htp#HiTOP-T01W1E"/>
        <rdfs:domain rdf:resource="http://purl.org/htp#HiTOP-T01XQi"/>
        <rdfs:domain rdf:resource="http://purl.org/htp#HiTOP-T01Y7w"/>
        <rdfs:domain rdf:resource="http://purl.org/htp#HiTOP-T01Ziz"/>
        <rdfs:domain rdf:resource="http://purl.org/htp#HiTOP-T01a7u"/>
        <rdfs:domain rdf:resource="http://purl.org/htp#HiTOP-T01bz7"/>
        <rdfs:domain rdf:resource="http://purl.org/htp#HiTOP-T01cX5"/>
        <rdfs:domain rdf:resource="http://purl.org/htp#HiTOP-T01d9I"/>
        <rdfs:domain rdf:resource="http://purl.org/htp#HiTOP-T01eG6"/>
        <rdfs:domain rdf:resource="http://purl.org/htp#HiTOP-T01fc8"/>
        <rdfs:domain rdf:resource="http://purl.org/htp#HiTOP-T01gKP"/>
        <rdfs:domain rdf:resource="http://purl.org/htp#HiTOP-U0012Y"/>
        <rdfs:domain rdf:resource="http://purl.org/htp#HiTOP-U002SC"/>
        <rdfs:domain rdf:resource="http://purl.org/htp#HiTOP-U0036N"/>
        <rdfs:domain rdf:resource="http://purl.org/htp#HiTOP-U004dm"/>
        <rdfs:domain rdf:resource="http://purl.org/htp#HiTOP-U005q"/>
        <rdfs:domain rdf:resource="http://purl.org/htp#HiTOP-U0061L"/>
        <rdfs:domain rdf:resource="http://purl.org/htp#HiTOP-U007EJ"/>
        <rdfs:domain rdf:resource="http://www.w3.org/1999/02/22-rdf-syntax-ns#DatatypeProperty"/>
        <rdfs:range rdf:resource="http://www.w3.org/2001/XMLSchema#string"/>
        <rdfs:comment xml:lang="en">A property used to specify the version ID, such as &quot;1.0&quot;, &quot;2.0&quot;, etc.</rdfs:comment>
        <rdfs:isDefinedBy rdf:resource="http://purl.org/htp#"/>
        <rdfs:label xml:lang="en">Has Version ID</rdfs:label>
    </owl:DatatypeProperty>
    


    <!-- http://purl.org/htp#versionDescription -->

    <owl:DatatypeProperty rdf:about="http://purl.org/htp#versionDescription">
        <rdfs:domain rdf:resource="http://purl.org/htp#HiTOP-C001qy"/>
        <rdfs:domain rdf:resource="http://purl.org/htp#HiTOP-C00217"/>
        <rdfs:domain rdf:resource="http://purl.org/htp#HiTOP-C0033z"/>
        <rdfs:domain rdf:resource="http://purl.org/htp#HiTOP-C00416"/>
        <rdfs:domain rdf:resource="http://purl.org/htp#HiTOP-C005Sv"/>
        <rdfs:domain rdf:resource="http://purl.org/htp#HiTOP-C006MD"/>
        <rdfs:domain rdf:resource="http://purl.org/htp#HiTOP-C00JTU"/>
        <rdfs:domain rdf:resource="http://purl.org/htp#HiTOP-C00KL0"/>
        <rdfs:domain rdf:resource="http://purl.org/htp#HiTOP-C00LqY"/>
        <rdfs:domain rdf:resource="http://purl.org/htp#HiTOP-C00Mpl"/>
        <rdfs:domain rdf:resource="http://purl.org/htp#HiTOP-C00N4I"/>
        <rdfs:domain rdf:resource="http://purl.org/htp#HiTOP-C00OuR"/>
        <rdfs:domain rdf:resource="http://purl.org/htp#HiTOP-C00Pjp"/>
        <rdfs:domain rdf:resource="http://purl.org/htp#HiTOP-C00Q1t"/>
        <rdfs:domain rdf:resource="http://purl.org/htp#HiTOP-C00RGy"/>
        <rdfs:domain rdf:resource="http://purl.org/htp#HiTOP-C00S9m"/>
        <rdfs:domain rdf:resource="http://purl.org/htp#HiTOP-C00TgL"/>
        <rdfs:domain rdf:resource="http://purl.org/htp#HiTOP-C00Urw"/>
        <rdfs:domain rdf:resource="http://purl.org/htp#HiTOP-C00VHv"/>
        <rdfs:domain rdf:resource="http://purl.org/htp#HiTOP-C00WJc"/>
        <rdfs:domain rdf:resource="http://purl.org/htp#HiTOP-C00XyI"/>
        <rdfs:domain rdf:resource="http://purl.org/htp#HiTOP-C00Y8j"/>
        <rdfs:domain rdf:resource="http://purl.org/htp#HiTOP-C00ZyP"/>
        <rdfs:domain rdf:resource="http://purl.org/htp#HiTOP-C00aMF"/>
        <rdfs:domain rdf:resource="http://purl.org/htp#HiTOP-C00bEx"/>
        <rdfs:domain rdf:resource="http://purl.org/htp#HiTOP-C00cSn"/>
        <rdfs:domain rdf:resource="http://purl.org/htp#HiTOP-C00dc1"/>
        <rdfs:domain rdf:resource="http://purl.org/htp#HiTOP-C00eL"/>
        <rdfs:domain rdf:resource="http://purl.org/htp#HiTOP-C00fKQ"/>
        <rdfs:domain rdf:resource="http://purl.org/htp#HiTOP-C00gvD"/>
        <rdfs:domain rdf:resource="http://purl.org/htp#HiTOP-C00hPJ"/>
        <rdfs:domain rdf:resource="http://purl.org/htp#HiTOP-C00iAh"/>
        <rdfs:domain rdf:resource="http://purl.org/htp#HiTOP-C00jw5"/>
        <rdfs:domain rdf:resource="http://purl.org/htp#HiTOP-C00kEN"/>
        <rdfs:domain rdf:resource="http://purl.org/htp#HiTOP-C00l5y"/>
        <rdfs:domain rdf:resource="http://purl.org/htp#HiTOP-C00mpe"/>
        <rdfs:domain rdf:resource="http://purl.org/htp#HiTOP-C00nyb"/>
        <rdfs:domain rdf:resource="http://purl.org/htp#HiTOP-C00oKM"/>
        <rdfs:domain rdf:resource="http://purl.org/htp#HiTOP-C00pnZ"/>
        <rdfs:domain rdf:resource="http://purl.org/htp#HiTOP-C00qSD"/>
        <rdfs:domain rdf:resource="http://purl.org/htp#HiTOP-C00rnS"/>
        <rdfs:domain rdf:resource="http://purl.org/htp#HiTOP-C00sWr"/>
        <rdfs:domain rdf:resource="http://purl.org/htp#HiTOP-C00tUQ"/>
        <rdfs:domain rdf:resource="http://purl.org/htp#HiTOP-C01DAb"/>
        <rdfs:domain rdf:resource="http://purl.org/htp#HiTOP-C01Elz"/>
        <rdfs:domain rdf:resource="http://purl.org/htp#HiTOP-C01FDy"/>
        <rdfs:domain rdf:resource="http://purl.org/htp#HiTOP-C01GEY"/>
        <rdfs:domain rdf:resource="http://purl.org/htp#HiTOP-C01HGq"/>
        <rdfs:domain rdf:resource="http://purl.org/htp#HiTOP-C01Ip4"/>
        <rdfs:domain rdf:resource="http://purl.org/htp#HiTOP-C01JH8"/>
        <rdfs:domain rdf:resource="http://purl.org/htp#HiTOP-C01KXo"/>
        <rdfs:domain rdf:resource="http://purl.org/htp#HiTOP-C01LSp"/>
        <rdfs:domain rdf:resource="http://purl.org/htp#HiTOP-C01MjB"/>
        <rdfs:domain rdf:resource="http://purl.org/htp#HiTOP-F001Hw"/>
        <rdfs:domain rdf:resource="http://purl.org/htp#HiTOP-P001Y2"/>
        <rdfs:domain rdf:resource="http://purl.org/htp#HiTOP-P002nf"/>
        <rdfs:domain rdf:resource="http://purl.org/htp#HiTOP-P003SL"/>
        <rdfs:domain rdf:resource="http://purl.org/htp#HiTOP-P004R1"/>
        <rdfs:domain rdf:resource="http://purl.org/htp#HiTOP-P005xY"/>
        <rdfs:domain rdf:resource="http://purl.org/htp#HiTOP-P006gM"/>
        <rdfs:domain rdf:resource="http://purl.org/htp#HiTOP-T007eM"/>
        <rdfs:domain rdf:resource="http://purl.org/htp#HiTOP-T008mD"/>
        <rdfs:domain rdf:resource="http://purl.org/htp#HiTOP-T0094I"/>
        <rdfs:domain rdf:resource="http://purl.org/htp#HiTOP-T00AZ"/>
        <rdfs:domain rdf:resource="http://purl.org/htp#HiTOP-T00BXK"/>
        <rdfs:domain rdf:resource="http://purl.org/htp#HiTOP-T00Cgy"/>
        <rdfs:domain rdf:resource="http://purl.org/htp#HiTOP-T00D42"/>
        <rdfs:domain rdf:resource="http://purl.org/htp#HiTOP-T00Eht"/>
        <rdfs:domain rdf:resource="http://purl.org/htp#HiTOP-T00Fe0"/>
        <rdfs:domain rdf:resource="http://purl.org/htp#HiTOP-T00G3d"/>
        <rdfs:domain rdf:resource="http://purl.org/htp#HiTOP-T00HCy"/>
        <rdfs:domain rdf:resource="http://purl.org/htp#HiTOP-T00IAT"/>
        <rdfs:domain rdf:resource="http://purl.org/htp#HiTOP-T00ua9"/>
        <rdfs:domain rdf:resource="http://purl.org/htp#HiTOP-T00vjR"/>
        <rdfs:domain rdf:resource="http://purl.org/htp#HiTOP-T00wk6"/>
        <rdfs:domain rdf:resource="http://purl.org/htp#HiTOP-T00xLn"/>
        <rdfs:domain rdf:resource="http://purl.org/htp#HiTOP-T00yfU"/>
        <rdfs:domain rdf:resource="http://purl.org/htp#HiTOP-T00zDk"/>
        <rdfs:domain rdf:resource="http://purl.org/htp#HiTOP-T010c6"/>
        <rdfs:domain rdf:resource="http://purl.org/htp#HiTOP-T011K6"/>
        <rdfs:domain rdf:resource="http://purl.org/htp#HiTOP-T012QL"/>
        <rdfs:domain rdf:resource="http://purl.org/htp#HiTOP-T013F1"/>
        <rdfs:domain rdf:resource="http://purl.org/htp#HiTOP-T014BA"/>
        <rdfs:domain rdf:resource="http://purl.org/htp#HiTOP-T015o8"/>
        <rdfs:domain rdf:resource="http://purl.org/htp#HiTOP-T016k0"/>
        <rdfs:domain rdf:resource="http://purl.org/htp#HiTOP-T0177S"/>
        <rdfs:domain rdf:resource="http://purl.org/htp#HiTOP-T018ir"/>
        <rdfs:domain rdf:resource="http://purl.org/htp#HiTOP-T019Cj"/>
        <rdfs:domain rdf:resource="http://purl.org/htp#HiTOP-T01A5i"/>
        <rdfs:domain rdf:resource="http://purl.org/htp#HiTOP-T01BfQ"/>
        <rdfs:domain rdf:resource="http://purl.org/htp#HiTOP-T01C1W"/>
        <rdfs:domain rdf:resource="http://purl.org/htp#HiTOP-T01Neb"/>
        <rdfs:domain rdf:resource="http://purl.org/htp#HiTOP-T01OY2"/>
        <rdfs:domain rdf:resource="http://purl.org/htp#HiTOP-T01PMW"/>
        <rdfs:domain rdf:resource="http://purl.org/htp#HiTOP-T01QNN"/>
        <rdfs:domain rdf:resource="http://purl.org/htp#HiTOP-T01RYG"/>
        <rdfs:domain rdf:resource="http://purl.org/htp#HiTOP-T01SYW"/>
        <rdfs:domain rdf:resource="http://purl.org/htp#HiTOP-T01T3u"/>
        <rdfs:domain rdf:resource="http://purl.org/htp#HiTOP-T01UGN"/>
        <rdfs:domain rdf:resource="http://purl.org/htp#HiTOP-T01VXq"/>
        <rdfs:domain rdf:resource="http://purl.org/htp#HiTOP-T01W1E"/>
        <rdfs:domain rdf:resource="http://purl.org/htp#HiTOP-T01XQi"/>
        <rdfs:domain rdf:resource="http://purl.org/htp#HiTOP-T01Y7w"/>
        <rdfs:domain rdf:resource="http://purl.org/htp#HiTOP-T01Ziz"/>
        <rdfs:domain rdf:resource="http://purl.org/htp#HiTOP-T01a7u"/>
        <rdfs:domain rdf:resource="http://purl.org/htp#HiTOP-T01bz7"/>
        <rdfs:domain rdf:resource="http://purl.org/htp#HiTOP-T01cX5"/>
        <rdfs:domain rdf:resource="http://purl.org/htp#HiTOP-T01d9I"/>
        <rdfs:domain rdf:resource="http://purl.org/htp#HiTOP-T01eG6"/>
        <rdfs:domain rdf:resource="http://purl.org/htp#HiTOP-T01fc8"/>
        <rdfs:domain rdf:resource="http://purl.org/htp#HiTOP-T01gKP"/>
        <rdfs:domain rdf:resource="http://purl.org/htp#HiTOP-U0012Y"/>
        <rdfs:domain rdf:resource="http://purl.org/htp#HiTOP-U002SC"/>
        <rdfs:domain rdf:resource="http://purl.org/htp#HiTOP-U0036N"/>
        <rdfs:domain rdf:resource="http://purl.org/htp#HiTOP-U004dm"/>
        <rdfs:domain rdf:resource="http://purl.org/htp#HiTOP-U005q"/>
        <rdfs:domain rdf:resource="http://purl.org/htp#HiTOP-U0061L"/>
        <rdfs:domain rdf:resource="http://purl.org/htp#HiTOP-U007EJ"/>
        <rdfs:range rdf:resource="http://www.w3.org/2001/XMLSchema#string"/>
    </owl:DatatypeProperty>
    


    <!-- 
    ///////////////////////////////////////////////////////////////////////////////////////
    //
    // Classes
    //
    ///////////////////////////////////////////////////////////////////////////////////////
     -->

    


    <!-- http://purl.org/htp#HiTOP-C001qy -->

    <owl:Class rdf:about="http://purl.org/htp#HiTOP-C001qy">
        <rdfs:subClassOf rdf:resource="http://purl.org/htp#HiTOP-O002sP"/>
        <obo:iaoIAO_0000115 xml:lang="en">
            Conversion =def. a Somatoform which is characterized by the expression of psychological distress as neurological or 
            physical symptoms that are inconsistent with medical findings, reflecting unconscious processes underlying the 
            symptom presentation.
        </obo:iaoIAO_0000115>
    </owl:Class>
    


    <!-- http://purl.org/htp#HiTOP-C00217 -->

    <owl:Class rdf:about="http://purl.org/htp#HiTOP-C00217">
        <rdfs:subClassOf rdf:resource="http://purl.org/htp#HiTOP-O002sP"/>
        <obo:iaoIAO_0000115 xml:lang="en">
            Somatization =def. a Somatoform which is characterized by the expression of psychological distress through multiple, 
            recurrent physical symptoms that cannot be fully explained by medical conditions.
        </obo:iaoIAO_0000115>
    </owl:Class>
    


    <!-- http://purl.org/htp#HiTOP-C0033z -->

    <owl:Class rdf:about="http://purl.org/htp#HiTOP-C0033z">
        <rdfs:subClassOf rdf:resource="http://purl.org/htp#HiTOP-O002sP"/>
        <obo:iaoIAO_0000115 xml:lang="en">
            Malaise =def. a Somatoform which is characterized by a general feeling of discomfort, unease, or lack of well-being, 
            reflecting psychological distress manifesting as nonspecific physical symptoms.
        </obo:iaoIAO_0000115>
    </owl:Class>
    


    <!-- http://purl.org/htp#HiTOP-C00416 -->

    <owl:Class rdf:about="http://purl.org/htp#HiTOP-C00416">
        <rdfs:subClassOf rdf:resource="http://purl.org/htp#HiTOP-O002sP"/>
        <obo:iaoIAO_0000115 xml:lang="en">
            Head Pain =def. a Somatoform which is characterized by headaches or other forms of head pain that are not 
            fully attributable to identifiable medical causes, reflecting the expression of psychological distress 
            through somatic symptoms.
        </obo:iaoIAO_0000115>
    </owl:Class>
    


    <!-- http://purl.org/htp#HiTOP-C005Sv -->

    <owl:Class rdf:about="http://purl.org/htp#HiTOP-C005Sv">
        <rdfs:subClassOf rdf:resource="http://purl.org/htp#HiTOP-O002sP"/>
        <obo:iaoIAO_0000115 xml:lang="en">
            Gastrointestinal =def. a Somatoform which is characterized by gastrointestinal symptoms such as abdominal pain, 
            bloating, nausea, or altered bowel habits that cannot be fully explained by medical findings, 
            reflecting psychological distress expressed through digestive complaints.
        </obo:iaoIAO_0000115>
    </owl:Class>
    


    <!-- http://purl.org/htp#HiTOP-C006MD -->

    <owl:Class rdf:about="http://purl.org/htp#HiTOP-C006MD">
        <rdfs:subClassOf rdf:resource="http://purl.org/htp#HiTOP-O002sP"/>
        <obo:iaoIAO_0000115 xml:lang="en">
            Cognitive =def. a Somatoform which is characterized by cognitive symptoms or dysfunctions such as difficulties 
            with memory, attention, or concentration, that are not fully explained by medical or neurological conditions, 
            reflecting psychological distress manifesting in cognitive domains.
        </obo:iaoIAO_0000115>
    </owl:Class>
    


    <!-- http://purl.org/htp#HiTOP-C00JTU -->

    <owl:Class rdf:about="http://purl.org/htp#HiTOP-C00JTU">
        <rdfs:subClassOf rdf:resource="http://purl.org/htp#HiTOP-O002sP"/>
        <obo:iaoIAO_0000115 xml:lang="en">
            Interactive Anxiety =def. a Fear which is characterized by anxiety experienced in social interactions and 
            group settings, often involving concerns about being judged, embarrassed, or negatively evaluated by others.
        </obo:iaoIAO_0000115>
    </owl:Class>
    


    <!-- http://purl.org/htp#HiTOP-C00KL0 -->

    <owl:Class rdf:about="http://purl.org/htp#HiTOP-C00KL0">
        <rdfs:subClassOf rdf:resource="http://purl.org/htp#HiTOP-O002sP"/>
        <obo:iaoIAO_0000115 xml:lang="en">
            Performance Anxiety =def. a Fear which is characterized by anxiety related to performing tasks or activities, 
            particularly in public or under observation, often driven by fear of failure, embarrassment, or negative evaluation.
        </obo:iaoIAO_0000115>
    </owl:Class>
    


    <!-- http://purl.org/htp#HiTOP-C00LqY -->

    <owl:Class rdf:about="http://purl.org/htp#HiTOP-C00LqY">
        <rdfs:subClassOf rdf:resource="http://purl.org/htp#HiTOP-O002sP"/>
        <obo:iaoIAO_0000115 xml:lang="en">
            Public Places =def. a Fear which is characterized by fear or anxiety associated with being in public spaces, 
            often involving concern about escape or access to help in case of distress.
        </obo:iaoIAO_0000115>
    </owl:Class>
    


    <!-- http://purl.org/htp#HiTOP-C00Mpl -->

    <owl:Class rdf:about="http://purl.org/htp#HiTOP-C00Mpl">
        <rdfs:subClassOf rdf:resource="http://purl.org/htp#HiTOP-O002sP"/>
        <obo:iaoIAO_0000115 xml:lang="en">
            Enclosed Spaces =def. a Fear which is characterized by fear or anxiety related to confined or small spaces, 
            often involving concerns about restriction, suffocation, or inability to escape.
        </obo:iaoIAO_0000115>
    </owl:Class>
    


    <!-- http://purl.org/htp#HiTOP-C00N4I -->

    <owl:Class rdf:about="http://purl.org/htp#HiTOP-C00N4I">
        <rdfs:subClassOf rdf:resource="http://purl.org/htp#HiTOP-O002sP"/>
        <obo:iaoIAO_0000115 xml:lang="en">
            Animal Phobia =def. a Fear which is characterized by fear or anxiety related to animals, 
            often involving specific triggers such as dogs, insects, or snakes, and resulting in avoidance behavior or 
            intense distress upon exposure.
        </obo:iaoIAO_0000115>
    </owl:Class>
    


    <!-- http://purl.org/htp#HiTOP-C00OuR -->

    <owl:Class rdf:about="http://purl.org/htp#HiTOP-C00OuR">
        <rdfs:subClassOf rdf:resource="http://purl.org/htp#HiTOP-O002sP"/>
        <obo:iaoIAO_0000115 xml:lang="en">
            Situational Phobia =def. a Fear which is characterized by fear or anxiety related to specific situations 
            or environments, such as flying, driving, tunnels, or elevators, typically leading to avoidance or marked distress.
        </obo:iaoIAO_0000115>
    </owl:Class>
    


    <!-- http://purl.org/htp#HiTOP-C00Pjp -->

    <owl:Class rdf:about="http://purl.org/htp#HiTOP-C00Pjp">
        <rdfs:subClassOf rdf:resource="http://purl.org/htp#HiTOP-O002sP"/>
        <obo:iaoIAO_0000115 xml:lang="en">
            Blood-Injection-Injury =def. a Fear which is characterized by fear or anxiety related to blood, injections, 
            or injuries, often accompanied by physiological responses such as fainting or nausea and resulting in 
            avoidance of medical procedures or traumatic stimuli.
        </obo:iaoIAO_0000115>
    </owl:Class>
    


    <!-- http://purl.org/htp#HiTOP-C00Q1t -->

    <owl:Class rdf:about="http://purl.org/htp#HiTOP-C00Q1t">
        <rdfs:subClassOf rdf:resource="http://purl.org/htp#HiTOP-O002sP"/>
        <obo:iaoIAO_0000115 xml:lang="en">
            Physiological Panic =def. a Fear which is characterized by sudden episodes of intense anxiety accompanied by 
            physiological symptoms such as rapid heartbeat, sweating, shortness of breath, or dizziness, 
            reflecting acute autonomic arousal.
        </obo:iaoIAO_0000115>
    </owl:Class>
    


    <!-- http://purl.org/htp#HiTOP-C00RGy -->

    <owl:Class rdf:about="http://purl.org/htp#HiTOP-C00RGy">
        <rdfs:subClassOf rdf:resource="http://purl.org/htp#HiTOP-O002sP"/>
        <obo:iaoIAO_0000115 xml:lang="en">
            Psychological Panic =def. a Fear which is characterized by an intense and overwhelming sense of fear accompanied 
            by cognitive symptoms such as a perceived loss of control, fear of going crazy, or impending doom, 
            often triggering physical reactions.
        </obo:iaoIAO_0000115>
    </owl:Class>
    


    <!-- http://purl.org/htp#HiTOP-C00S9m -->

    <owl:Class rdf:about="http://purl.org/htp#HiTOP-C00S9m">
        <rdfs:subClassOf rdf:resource="http://purl.org/htp#HiTOP-O002sP"/>
        <obo:iaoIAO_0000115 xml:lang="en">
            Cleaning =def. a Fear which is characterized by compulsive behaviors related to cleaning or hygiene, 
            typically performed to reduce anxiety about contamination or illness.
        </obo:iaoIAO_0000115>
    </owl:Class>
    


    <!-- http://purl.org/htp#HiTOP-C00TgL -->

    <owl:Class rdf:about="http://purl.org/htp#HiTOP-C00TgL">
        <rdfs:subClassOf rdf:resource="http://purl.org/htp#HiTOP-O002sP"/>
        <obo:iaoIAO_0000115 xml:lang="en">
            Rituals =def. a Fear which is characterized by compulsive behaviors or mental acts performed in a specific and 
            repetitive manner, typically intended to prevent feared outcomes or reduce anxiety.
        </obo:iaoIAO_0000115>
    </owl:Class>
    


    <!-- http://purl.org/htp#HiTOP-C00Urw -->

    <owl:Class rdf:about="http://purl.org/htp#HiTOP-C00Urw">
        <rdfs:subClassOf rdf:resource="http://purl.org/htp#HiTOP-O002sP"/>
        <obo:iaoIAO_0000115 xml:lang="en">
            Checking =def. a Fear which is characterized by compulsive behaviors involving repeated checking of objects or 
            situations—such as locks, appliances, or personal belongings—typically performed to reduce anxiety about 
            potential harm or danger.
        </obo:iaoIAO_0000115>
    </owl:Class>
    


    <!-- http://purl.org/htp#HiTOP-C00VHv -->

    <owl:Class rdf:about="http://purl.org/htp#HiTOP-C00VHv">
        <rdfs:subClassOf rdf:resource="http://purl.org/htp#HiTOP-O002sP"/>
        <obo:iaoIAO_0000115 xml:lang="en">
            Dysphoria =def. a Distress which is characterized by a generalized state of unhappiness, dissatisfaction, 
            or emotional discomfort, often involving irritability, restlessness, or low mood without a specific cause.
        </obo:iaoIAO_0000115>
    </owl:Class>
    


    <!-- http://purl.org/htp#HiTOP-C00WJc -->

    <owl:Class rdf:about="http://purl.org/htp#HiTOP-C00WJc">
        <rdfs:subClassOf rdf:resource="http://purl.org/htp#HiTOP-O002sP"/>
        <obo:iaoIAO_0000115 xml:lang="en">
            Lassitude =def. a Distress which is characterized by physical or mental weariness and a lack of energy, 
            often accompanied by reduced motivation, sluggishness, or difficulty initiating tasks.
        </obo:iaoIAO_0000115>
    </owl:Class>
    


    <!-- http://purl.org/htp#HiTOP-C00XyI -->

    <owl:Class rdf:about="http://purl.org/htp#HiTOP-C00XyI">
        <rdfs:subClassOf rdf:resource="http://purl.org/htp#HiTOP-O002sP"/>
        <obo:iaoIAO_0000115 xml:lang="en">
            Anhedonia =def. a Distress which is characterized by a diminished ability to experience interest or pleasure 
            in activities that are typically found enjoyable, reflecting a core symptom of depressive states.
        </obo:iaoIAO_0000115>
    </owl:Class>
    


    <!-- http://purl.org/htp#HiTOP-C00Y8j -->

    <owl:Class rdf:about="http://purl.org/htp#HiTOP-C00Y8j">
        <rdfs:subClassOf rdf:resource="http://purl.org/htp#HiTOP-O002sP"/>
        <obo:iaoIAO_0000115 xml:lang="en">
            Insomnia =def. a Distress which is characterized by difficulty falling asleep, staying asleep, or waking too 
            early and being unable to return to sleep, often resulting in daytime fatigue, irritability, or impaired functioning.
        </obo:iaoIAO_0000115>
    </owl:Class>
    


    <!-- http://purl.org/htp#HiTOP-C00ZyP -->

    <owl:Class rdf:about="http://purl.org/htp#HiTOP-C00ZyP">
        <rdfs:subClassOf rdf:resource="http://purl.org/htp#HiTOP-O002sP"/>
        <obo:iaoIAO_0000115 xml:lang="en">
            Suicidality =def. a Distress which is characterized by the presence of thoughts, intentions, or behaviors 
            related to ending one’s own life, often associated with severe emotional suffering and hopelessness.
        </obo:iaoIAO_0000115>
    </owl:Class>
    


    <!-- http://purl.org/htp#HiTOP-C00aMF -->

    <owl:Class rdf:about="http://purl.org/htp#HiTOP-C00aMF">
        <rdfs:subClassOf rdf:resource="http://purl.org/htp#HiTOP-O002sP"/>
        <obo:iaoIAO_0000115 xml:lang="en">
            Agitation =def. a Distress which is characterized by a state of heightened emotional or physiological arousal, 
            often resulting in restlessness, irritability, or erratic behavior.
        </obo:iaoIAO_0000115>
    </owl:Class>
    


    <!-- http://purl.org/htp#HiTOP-C00bEx -->

    <owl:Class rdf:about="http://purl.org/htp#HiTOP-C00bEx">
        <rdfs:subClassOf rdf:resource="http://purl.org/htp#HiTOP-O002sP"/>
        <obo:iaoIAO_0000115 xml:lang="en">
            Retardation =def. a Distress which is characterized by slowed cognitive and physical processes, including delays 
            in thinking, speaking, and moving, often observed in depressive states.
        </obo:iaoIAO_0000115>
    </owl:Class>
    


    <!-- http://purl.org/htp#HiTOP-C00cSn -->

    <owl:Class rdf:about="http://purl.org/htp#HiTOP-C00cSn">
        <rdfs:subClassOf rdf:resource="http://purl.org/htp#HiTOP-O002sP"/>
        <obo:iaoIAO_0000115 xml:lang="en">
            Appetite Loss =def. a Distress which is characterized by a reduction or loss of desire to eat, 
            often resulting in decreased food intake and potential weight loss, commonly associated with depressive or 
            anxious states.
        </obo:iaoIAO_0000115>
    </owl:Class>
    


    <!-- http://purl.org/htp#HiTOP-C00dc1 -->

    <owl:Class rdf:about="http://purl.org/htp#HiTOP-C00dc1">
        <rdfs:subClassOf rdf:resource="http://purl.org/htp#HiTOP-O002sP"/>
        <obo:iaoIAO_0000115 xml:lang="en">
            Appetite Gain =def. a Distress which is characterized by an increased desire to eat, often resulting in 
            elevated food intake and potential weight gain, commonly observed in atypical depressive states or in response 
            to emotional distress.
        </obo:iaoIAO_0000115>
    </owl:Class>
    


    <!-- http://purl.org/htp#HiTOP-C00eL -->

    <owl:Class rdf:about="http://purl.org/htp#HiTOP-C00eL">
        <rdfs:subClassOf rdf:resource="http://purl.org/htp#HiTOP-O002sP"/>
        <obo:iaoIAO_0000115 xml:lang="en">
            (low) Wellbeing =def. a Distress which is characterized by a diminished state of mental and physical health, 
            reflected in reduced happiness, life satisfaction, or emotional balance.
        </obo:iaoIAO_0000115>
    </owl:Class>
    


    <!-- http://purl.org/htp#HiTOP-C00fKQ -->

    <owl:Class rdf:about="http://purl.org/htp#HiTOP-C00fKQ">
        <rdfs:subClassOf rdf:resource="http://purl.org/htp#HiTOP-O002sP"/>
        <obo:iaoIAO_0000115 xml:lang="en">
            Generalized Anxiety Disorder Symptoms =def. a Distress which is characterized by excessive and persistent worry 
            that interferes with daily functioning, often accompanied by physical symptoms such as restlessness, fatigue, 
            and muscle tension.
        </obo:iaoIAO_0000115>
    </owl:Class>
    


    <!-- http://purl.org/htp#HiTOP-C00gvD -->

    <owl:Class rdf:about="http://purl.org/htp#HiTOP-C00gvD">
        <rdfs:subClassOf rdf:resource="http://purl.org/htp#HiTOP-O002sP"/>
        <obo:iaoIAO_0000115 xml:lang="en">
            Re-experiencing =def. a Distress which is characterized by the involuntary re-living of traumatic events through 
            flashbacks, intrusive memories, or nightmares, often accompanied by intense emotional or physiological reactions.
        </obo:iaoIAO_0000115>
    </owl:Class>
    


    <!-- http://purl.org/htp#HiTOP-C00hPJ -->

    <owl:Class rdf:about="http://purl.org/htp#HiTOP-C00hPJ">
        <rdfs:subClassOf rdf:resource="http://purl.org/htp#HiTOP-O002sP"/>
        <obo:iaoIAO_0000115 xml:lang="en">
            Avoidance =def. a Distress which is characterized by efforts to avoid thoughts, feelings, people, places, 
            or situations that are associated with traumatic experiences or stress, often as a means of reducing 
            emotional discomfort or fear.
        </obo:iaoIAO_0000115>
    </owl:Class>
    


    <!-- http://purl.org/htp#HiTOP-C00iAh -->

    <owl:Class rdf:about="http://purl.org/htp#HiTOP-C00iAh">
        <rdfs:subClassOf rdf:resource="http://purl.org/htp#HiTOP-O002sP"/>
        <obo:iaoIAO_0000115 xml:lang="en">
            Hyperarousal =def. a Distress which is characterized by increased physiological arousal, including symptoms such as 
            hypervigilance, irritability, exaggerated startle response, and difficulty sleeping, often associated with 
            trauma-related or anxiety disorders.
        </obo:iaoIAO_0000115>
    </owl:Class>
    


    <!-- http://purl.org/htp#HiTOP-C00jw5 -->

    <owl:Class rdf:about="http://purl.org/htp#HiTOP-C00jw5">
        <rdfs:subClassOf rdf:resource="http://purl.org/htp#HiTOP-O002sP"/>
        <obo:iaoIAO_0000115 xml:lang="en">
            Numbing =def. a Distress which is characterized by emotional numbness or detachment from feelings, 
            typically as a psychological response to overwhelming stress or trauma, and often accompanied by 
            a diminished capacity to experience positive emotions.
        </obo:iaoIAO_0000115>
    </owl:Class>
    


    <!-- http://purl.org/htp#HiTOP-C00kEN -->

    <owl:Class rdf:about="http://purl.org/htp#HiTOP-C00kEN">
        <rdfs:subClassOf rdf:resource="http://purl.org/htp#HiTOP-O002sP"/>
        <obo:iaoIAO_0000115 xml:lang="en">
            Dissociation =def. a Distress which is characterized by a mental process used to cope with stress or trauma, 
            leading to a sense of detachment from one’s surroundings, identity, or sense of self, and often resulting in 
            altered perception or memory.
        </obo:iaoIAO_0000115>
    </owl:Class>
    


    <!-- http://purl.org/htp#HiTOP-C00l5y -->

    <owl:Class rdf:about="http://purl.org/htp#HiTOP-C00l5y">
        <rdfs:subClassOf rdf:resource="http://purl.org/htp#HiTOP-O002sP"/>
        <obo:iaoIAO_0000115 xml:lang="en">
            Irritability =def. a Distress which is characterized by a heightened tendency to become easily annoyed or angered, 
            often involving a low tolerance for frustration and frequent mood outbursts.
        </obo:iaoIAO_0000115>
    </owl:Class>
    


    <!-- http://purl.org/htp#HiTOP-C00mpe -->

    <owl:Class rdf:about="http://purl.org/htp#HiTOP-C00mpe">
        <rdfs:subClassOf rdf:resource="http://purl.org/htp#HiTOP-O002sP"/>
        <obo:iaoIAO_0000115 xml:lang="en">
            Pure Obsessions =def. a Distress which is characterized by recurrent and persistent intrusive thoughts, images, 
            or impulses that cause significant distress, without being accompanied by observable compulsive behaviors intended 
            to neutralize them.
        </obo:iaoIAO_0000115>
    </owl:Class>
    


    <!-- http://purl.org/htp#HiTOP-C00nyb -->

    <owl:Class rdf:about="http://purl.org/htp#HiTOP-C00nyb">
        <rdfs:subClassOf rdf:resource="http://purl.org/htp#HiTOP-O002sP"/>
        <obo:iaoIAO_0000115 xml:lang="en">
            Euphoric Activation =def. a Mania which is characterized by heightened mood, increased energy, and elevated 
            self-confidence, often associated with euphoric or expansive affect seen in manic or hypomanic episodes.
        </obo:iaoIAO_0000115>
    </owl:Class>
    


    <!-- http://purl.org/htp#HiTOP-C00oKM -->

    <owl:Class rdf:about="http://purl.org/htp#HiTOP-C00oKM">
        <rdfs:subClassOf rdf:resource="http://purl.org/htp#HiTOP-O002sP"/>
        <obo:iaoIAO_0000115 xml:lang="en">
            Hyperactive Cognition =def. a Mania which is characterized by increased cognitive activity, including racing thoughts, 
            distractibility, and accelerated ideation, often leading to difficulties in concentration and goal-directed thinking.
        </obo:iaoIAO_0000115>
    </owl:Class>
    


    <!-- http://purl.org/htp#HiTOP-C00pnZ -->

    <owl:Class rdf:about="http://purl.org/htp#HiTOP-C00pnZ">
        <rdfs:subClassOf rdf:resource="http://purl.org/htp#HiTOP-O002sP"/>
        <obo:iaoIAO_0000115 xml:lang="en">
            Reckless Overconfidence =def. a Mania which is characterized by excessive self-confidence that leads to risky, 
            impulsive, or poorly judged behaviors, often without regard for potential negative consequences, as 
            commonly observed in manic episodes.
        </obo:iaoIAO_0000115>
    </owl:Class>
    


    <!-- http://purl.org/htp#HiTOP-C00qSD -->

    <owl:Class rdf:about="http://purl.org/htp#HiTOP-C00qSD">
        <rdfs:subClassOf rdf:resource="http://purl.org/htp#HiTOP-O002sP"/>
        <obo:iaoIAO_0000115 xml:lang="en">
            Psychotic =def. a Thought Disorder which is characterized by symptoms of psychosis, such as delusions, 
            hallucinations, disorganized thinking, or impaired reality testing.
        </obo:iaoIAO_0000115>
    </owl:Class>
    


    <!-- http://purl.org/htp#HiTOP-C00rnS -->

    <owl:Class rdf:about="http://purl.org/htp#HiTOP-C00rnS">
        <rdfs:subClassOf rdf:resource="http://purl.org/htp#HiTOP-O002sP"/>
        <obo:iaoIAO_0000115 xml:lang="en">
            Disorganized =def. a Thought Disorder which is characterized by disorganized thinking and behavior, 
            including incoherent speech, erratic actions, and difficulties maintaining goal-directed activity.
        </obo:iaoIAO_0000115>
    </owl:Class>
    


    <!-- http://purl.org/htp#HiTOP-C00sWr -->

    <owl:Class rdf:about="http://purl.org/htp#HiTOP-C00sWr">
        <rdfs:subClassOf rdf:resource="http://purl.org/htp#HiTOP-O002sP"/>
        <obo:iaoIAO_0000115 xml:lang="en">
            Inexpressivity =def. a Thought Disorder which is characterized by a lack of emotional expression, including reduced 
            facial expressions, vocal inflection, and gestures, often observed as a negative symptom in psychotic disorders.
        </obo:iaoIAO_0000115>
    </owl:Class>
    


    <!-- http://purl.org/htp#HiTOP-C00tUQ -->

    <owl:Class rdf:about="http://purl.org/htp#HiTOP-C00tUQ">
        <rdfs:subClassOf rdf:resource="http://purl.org/htp#HiTOP-O002sP"/>
        <obo:iaoIAO_0000115 xml:lang="en">
            Avolition =def. a Thought Disorder which is characterized by a lack of motivation to initiate and sustain purposeful 
            activities, often resulting in reduced goal-directed behavior and functional impairment in daily life.
        </obo:iaoIAO_0000115>
    </owl:Class>
    


    <!-- http://purl.org/htp#HiTOP-C01DAb -->

    <owl:Class rdf:about="http://purl.org/htp#HiTOP-C01DAb">
        <rdfs:subClassOf rdf:resource="http://purl.org/htp#HiTOP-O002sP"/>
        <obo:iaoIAO_0000115 xml:lang="en">
            Alcohol Use =def. a Harmful Substance Abuse which is characterized by the consumption of alcoholic beverages, 
            which may lead to problematic use, dependence, or negative physical, psychological, or social consequences.
        </obo:iaoIAO_0000115>
    </owl:Class>
    


    <!-- http://purl.org/htp#HiTOP-C01Elz -->

    <owl:Class rdf:about="http://purl.org/htp#HiTOP-C01Elz">
        <rdfs:subClassOf rdf:resource="http://purl.org/htp#HiTOP-O002sP"/>
        <obo:iaoIAO_0000115 xml:lang="en">
            Alcohol Problems =def. a Harmful Substance Abuse which is characterized by issues related to the use of alcohol, 
            including dependence, abuse, and the negative physical, psychological, and social consequences resulting from 
            excessive consumption.
        </obo:iaoIAO_0000115>
    </owl:Class>
    


    <!-- http://purl.org/htp#HiTOP-C01FDy -->

    <owl:Class rdf:about="http://purl.org/htp#HiTOP-C01FDy">
        <rdfs:subClassOf rdf:resource="http://purl.org/htp#HiTOP-O002sP"/>
        <obo:iaoIAO_0000115 xml:lang="en">
            Marijuana Use =def. a Harmful Substance Abuse which is characterized by the consumption of marijuana, 
            which may lead to problematic use, dependence, or negative physical, psychological, or social consequences.
        </obo:iaoIAO_0000115>
    </owl:Class>
    


    <!-- http://purl.org/htp#HiTOP-C01GEY -->

    <owl:Class rdf:about="http://purl.org/htp#HiTOP-C01GEY">
        <rdfs:subClassOf rdf:resource="http://purl.org/htp#HiTOP-O002sP"/>
        <obo:iaoIAO_0000115 xml:lang="en">
            Marijuana Problems =def. a Harmful Substance Abuse which is characterized by issues related to the use of marijuana, 
            including dependence, abuse, and the negative physical, psychological, and social consequences resulting from 
            excessive consumption.
        </obo:iaoIAO_0000115>
    </owl:Class>
    


    <!-- http://purl.org/htp#HiTOP-C01HGq -->

    <owl:Class rdf:about="http://purl.org/htp#HiTOP-C01HGq">
        <rdfs:subClassOf rdf:resource="http://purl.org/htp#HiTOP-O002sP"/>
        <obo:iaoIAO_0000115 xml:lang="en">
            Drug Use =def. a Harmful Substance Abuse which is characterized by the consumption of illicit or prescription drugs, 
            which may lead to problematic use, dependence, or negative physical, psychological, or social consequences.
        </obo:iaoIAO_0000115>
    </owl:Class>
    


    <!-- http://purl.org/htp#HiTOP-C01Ip4 -->

    <owl:Class rdf:about="http://purl.org/htp#HiTOP-C01Ip4">
        <rdfs:subClassOf rdf:resource="http://purl.org/htp#HiTOP-O002sP"/>
        <obo:iaoIAO_0000115 xml:lang="en">
            Drug Problems =def. a Harmful Substance Abuse which is characterized by issues related to the use of drugs, 
            including dependence, abuse, and the negative physical, psychological, and social consequences resulting from 
            excessive or harmful consumption.
        </obo:iaoIAO_0000115>
    </owl:Class>
    


    <!-- http://purl.org/htp#HiTOP-C01JH8 -->

    <owl:Class rdf:about="http://purl.org/htp#HiTOP-C01JH8">
        <rdfs:subClassOf rdf:resource="http://purl.org/htp#HiTOP-O002sP"/>
        <obo:iaoIAO_0000115 xml:lang="en">
            Physical Aggression =def. an Antisocial Behavior which is characterized by the use of physical acts of 
            violence towards others, often involving harm or the threat of harm, and typically reflecting a disregard for 
            social norms and the rights of others.
        </obo:iaoIAO_0000115>
    </owl:Class>
    


    <!-- http://purl.org/htp#HiTOP-C01KXo -->

    <owl:Class rdf:about="http://purl.org/htp#HiTOP-C01KXo">
        <rdfs:subClassOf rdf:resource="http://purl.org/htp#HiTOP-O002sP"/>
        <obo:iaoIAO_0000115 xml:lang="en">
            Destructive Aggression =def. an Antisocial Behavior which is characterized by aggression that results in 
            damage to property or the environment, often reflecting a disregard for social norms, authority, or 
            the consequences of one’s actions.
        </obo:iaoIAO_0000115>
    </owl:Class>
    


    <!-- http://purl.org/htp#HiTOP-C01LSp -->

    <owl:Class rdf:about="http://purl.org/htp#HiTOP-C01LSp">
        <rdfs:subClassOf rdf:resource="http://purl.org/htp#HiTOP-O002sP"/>
        <obo:iaoIAO_0000115 xml:lang="en">
            Relational Aggression =def. an Antisocial Behavior which is characterized by aggression that harms others 
            through manipulation of social relationships, such as spreading rumors, social exclusion, or 
            undermining someone's reputation.
        </obo:iaoIAO_0000115>
    </owl:Class>
    


    <!-- http://purl.org/htp#HiTOP-C01MjB -->

    <owl:Class rdf:about="http://purl.org/htp#HiTOP-C01MjB">
        <rdfs:subClassOf rdf:resource="http://purl.org/htp#HiTOP-O002sP"/>
        <obo:iaoIAO_0000115 xml:lang="en">
            Fraud =def. an Antisocial Behavior which is characterized by deceptive behavior intended to secure unfair or 
            unlawful gain, often involving manipulation, dishonesty, or the misrepresentation of information to deceive others.
        </obo:iaoIAO_0000115>
    </owl:Class>
    


    <!-- http://purl.org/htp#HiTOP-F001Hw -->

    <owl:Class rdf:about="http://purl.org/htp#HiTOP-F001Hw">
        <rdfs:subClassOf rdf:resource="http://purl.org/htp#HiTOP-O002sP"/>
        <obo:iaoIAO_0000115 xml:lang="en">
            General Psychopathology = Def. a Psychological Condition which manifests across multiple 
            mental health disorders and includes broad symptoms such as mood disturbances, anxiety, 
            cognitive dysfunctions, and behavioral problems.
        </obo:iaoIAO_0000115>
        <rdfs:comment xml:lang="en">
            General Psychopathology refers to the broad, overarching category of mental disorders and 
            psychological symptoms that can manifest across different mental health conditions. It encompasses a wide range of 
            psychological phenomena that are not specific to any single disorder but may contribute to or exacerbate multiple types 
            of mental health issues. This category includes general symptoms and traits that are commonly observed in various 
            psychiatric conditions, such as mood disturbances, anxiety, cognitive dysfunctions, and behavioral problems.
        </rdfs:comment>
        <rdfs:label xml:lang="en">General Psychopathology</rdfs:label>
        <skos:changeNote>
            Indicates the potential for future inclusion of additional spectra and other related concepts as new developments and 
            insights emerge in the field of general psychopathology. Allows for flexible expansion and refinement of the taxonomy 
            to integrate new spectra, subfactors, and related elements to better capture evolving understanding and research 
            findings.
        </skos:changeNote>
    </owl:Class>
    


    <!-- http://purl.org/htp#HiTOP-O001Ih -->

    <owl:Class rdf:about="http://purl.org/htp#HiTOP-O001Ih">
        <rdfs:subClassOf>
            <owl:Restriction>
                <owl:onProperty rdf:resource="http://purl.org/htp#hasLevel"/>
                <owl:someValuesFrom rdf:resource="http://purl.org/htp#HiTOP-O001Ih"/>
            </owl:Restriction>
        </rdfs:subClassOf>
        <rdfs:comment xml:lang="en">
            A structural component of the HiTOP taxonomy used to define hierarchical relationships between psychological constructs. 
            Each instance of Level represents a specific position in the vertical hierarchy, encompassing constructs such as 
            psychopathology factors, superspectra, spectra, subfactors, and components.
            The restriction ensures that all instances of this class must 
            have at least one level (via the property htp:hasLevel) 
            that is also an instance of this class.
        </rdfs:comment>
        <rdfs:label xml:lang="en">Level</rdfs:label>
    </owl:Class>
    


    <!-- http://purl.org/htp#HiTOP-O002sP -->

    <owl:Class rdf:about="http://purl.org/htp#HiTOP-O002sP">
        <rdfs:subClassOf>
            <owl:Restriction>
                <owl:onProperty rdf:resource="http://purl.org/htp#hasTier"/>
                <owl:someValuesFrom rdf:resource="http://purl.org/htp#HiTOP-O002sP"/>
            </owl:Restriction>
        </rdfs:subClassOf>
        <rdfs:comment xml:lang="en">
            A structural component of the HiTOP taxonomy used to define horizontal relationships within a specific level of the hierarchy. 
            Each instance of Tier represents a distinct grouping or division within a given Level, encompassing constructs such as 
            clusters, categories, or subcategories. The restriction ensures that all instances of this class must have at least one tier 
            (via the property htp:hasTier) that is also an instance of this class.
        </rdfs:comment>
        <rdfs:label xml:lang="en">Tier</rdfs:label>
    </owl:Class>
    


    <!-- http://purl.org/htp#HiTOP-O003W -->

    <owl:Class rdf:about="http://purl.org/htp#HiTOP-O003W">
        <rdfs:subClassOf>
            <owl:Restriction>
                <owl:onProperty rdf:resource="http://purl.org/htp#hasFactor"/>
                <owl:someValuesFrom rdf:resource="http://purl.org/htp#HiTOP-O003W"/>
            </owl:Restriction>
        </rdfs:subClassOf>
        <rdfs:comment xml:lang="en">
            A core construct in the HiTOP framework that represents broad, underlying dimensions of psychopathology. 
            Factors are used to classify and diagnose mental health conditions, forming the highest level of the taxonomy.
        </rdfs:comment>
        <rdfs:label xml:lang="en">Factor</rdfs:label>
    </owl:Class>
    


    <!-- http://purl.org/htp#HiTOP-P001Y2 -->

    <owl:Class rdf:about="http://purl.org/htp#HiTOP-P001Y2">
        <rdfs:subClassOf rdf:resource="http://purl.org/htp#HiTOP-O002sP"/>
        <obo:iaoIAO_0000115 xml:lang="en">
            Somatoform =def. a General Psychopathology which is characterized by physical symptoms that cannot be fully explained 
            by a medical condition and reflect psychological distress expressed through somatic complaints.
        </obo:iaoIAO_0000115>
        <rdfs:comment xml:lang="en">
            The Somatoform label refers to a category of mental health disorders characterized by physical symptoms that cannot be 
            fully explained by any underlying medical condition, highlighting the complex interaction between mind and body in 
            mental health.
        </rdfs:comment>
        <rdfs:label xml:lang="en">Somatoform</rdfs:label>
        <skos:changeNote xml:lang="en">
            This spectrum may include future expansions or modifications based on emerging research or changes in the understanding of somatoform disorders. 
            It is designed to adapt to new developments by allowing the addition of new related spectra or concepts as needed.
        </skos:changeNote>
    </owl:Class>
    


    <!-- http://purl.org/htp#HiTOP-P002nf -->

    <owl:Class rdf:about="http://purl.org/htp#HiTOP-P002nf">
        <rdfs:subClassOf rdf:resource="http://purl.org/htp#HiTOP-O002sP"/>
        <obo:iaoIAO_0000115 xml:lang="en">
            Internalizing =def. a General Psychopathology which is characterized by inward-directed symptoms such as anxiety, 
            depression, and social withdrawal, indicating emotional and cognitive distress that is primarily internal in nature.
        </obo:iaoIAO_0000115>
        <rdfs:comment xml:lang="en">
            The Internalizing label refers to a category of mental health disorders characterized by inward-focused symptoms such as 
            anxiety, depression, and withdrawal, reflecting emotional and cognitive distress.
        </rdfs:comment>
        <rdfs:label xml:lang="en">Internalizing</rdfs:label>
        <skos:changeNote xml:lang="en">
            This spectrum can accommodate future additions or modifications based on emerging research or evolving understanding of internalizing disorders. 
            It is designed to integrate new related spectra or concepts as needed, reflecting the ongoing developments in the field.
        </skos:changeNote>
    </owl:Class>
    


    <!-- http://purl.org/htp#HiTOP-P003SL -->

    <owl:Class rdf:about="http://purl.org/htp#HiTOP-P003SL">
        <rdfs:subClassOf rdf:resource="http://purl.org/htp#HiTOP-O002sP"/>
        <obo:iaoIAO_0000115 xml:lang="en">
            Thought Disorder =def. a General Psychopathology which is characterized by disorganized thinking, 
            impaired reality testing, and disturbances in the form or content of thought, reflecting severe cognitive and 
            perceptual disruptions.
        </obo:iaoIAO_0000115>
        <rdfs:comment xml:lang="en">
            Thought Disorder refers to a category of mental health conditions characterized by disorganized thinking, impaired 
            reality testing, and disturbances in the form or content of thought.
        </rdfs:comment>
        <rdfs:label xml:lang="en">Thought Disorder</rdfs:label>
        <skos:changeNote xml:lang="en">
            This spectrum allows for the integration of additional related spectra or concepts as new insights into thought disorders emerge. 
            It is structured to adapt to evolving understandings and classifications within the domain of cognitive and thought-related disturbances.
        </skos:changeNote>
    </owl:Class>
    


    <!-- http://purl.org/htp#HiTOP-P004R1 -->

    <owl:Class rdf:about="http://purl.org/htp#HiTOP-P004R1">
        <rdfs:subClassOf rdf:resource="http://purl.org/htp#HiTOP-O002sP"/>
        <obo:iaoIAO_0000115 xml:lang="en">
            Detachment =def. a General Psychopathology which is characterized by emotional distance and disengagement 
            from social interactions, reflecting a reduced capacity for affective connection and interpersonal involvement.
        </obo:iaoIAO_0000115>
        <rdfs:comment xml:lang="en">
            Detachment refers to a psychological state characterized by emotional distance and disengagement from social interactions.
        </rdfs:comment>
        <rdfs:label xml:lang="en">Detachment</rdfs:label>
        <skos:changeNote xml:lang="en">
            This spectrum is designed to accommodate the inclusion of new related spectra or additional concepts as understanding of detachment and related psychological phenomena evolves. 
            It supports updates and extensions to reflect advances in research and shifts in diagnostic criteria.
        </skos:changeNote>
    </owl:Class>
    

    <!-- http://purl.org/htp#HiTOP-S0013h -->

    <owl:Class rdf:about="http://purl.org/htp#HiTOP-S0013h">
        <rdfs:subClassOf rdf:resource="http://purl.org/htp#HiTOP-O002sP"/>
        <obo:iaoIAO_0000115 xml:lang="en">
            Externalizing =def. a General Psychopathology which is characterized by outwardly directed behaviors and 
            dysregulation, including impulsivity, aggression, and rule-breaking actions that disrupt external environments.
        </obo:iaoIAO_0000115>
        <rdfs:comment xml:lang="en">
            Represents a broad HiTOP dimension characterized by outwardly directed behaviors and dysregulation.
        </rdfs:comment>
        <rdfs:label xml:lang="en">Externalizing</rdfs:label>
        <skos:changeNote xml:lang="en">
            This superspectrum is structured to support future refinements and extensions. 
            It allows for the incorporation of additional spectra or subdimensions to reflect ongoing developments 
            in the conceptualization and classification of externalizing behaviors and dysregulation.
        </skos:changeNote>
    </owl:Class>


    <!-- http://purl.org/htp#HiTOP-P005xY -->

    <owl:Class rdf:about="http://purl.org/htp#HiTOP-P005xY">
        <rdfs:subClassOf rdf:resource="http://purl.org/htp#HiTOP-O002sP"/>
        <obo:iaoIAO_0000115 xml:lang="en">
            Disinhibited Externalizing =def. an Externalizing which is characterized by impulsive behaviors and 
            a lack of social restraint or inhibition, reflecting difficulties in self-regulation and behavioral control.
        </obo:iaoIAO_0000115>
        <rdfs:comment xml:lang="en">
            Disinhibited Externalizing involves behaviors that are impulsive and lacking in social restraint or inhibition.
        </rdfs:comment>
        <rdfs:label xml:lang="en">Disinhibited Externalizing</rdfs:label>
        <skos:changeNote xml:lang="en">
            This spectrum is designed to be adaptable to the addition of new spectra or related concepts as research on disinhibited externalizing behaviors evolves. 
            It allows for updates and expansions to incorporate emerging findings and shifts in diagnostic frameworks.
        </skos:changeNote>
    </owl:Class>
    


    <!-- http://purl.org/htp#HiTOP-P006gM -->

    <owl:Class rdf:about="http://purl.org/htp#HiTOP-P006gM">
        <rdfs:subClassOf rdf:resource="http://purl.org/htp#HiTOP-O002sP"/>
        <obo:iaoIAO_0000115 xml:lang="en">
            Antagonistic Externalizing =def. an Externalizing which is characterized by hostile and 
            aggressive behaviors directed toward others, reflecting interpersonal antagonism and a tendency 
            to violate social norms or the rights of others.
        </obo:iaoIAO_0000115>
        <rdfs:comment xml:lang="en">
            Antagonistic Externalizing describes behaviors that involve hostility and aggression towards others.
        </rdfs:comment>
        <rdfs:label xml:lang="en">Antagonistic Externalizing</rdfs:label>
        <skos:changeNote xml:lang="en">
            This spectrum is designed to accommodate potential future modifications and expansions. 
            It supports the integration of new spectra or related concepts to reflect advancements in understanding antagonistic externalizing behaviors and their classification.
        </skos:changeNote>
    </owl:Class>
    


    <!-- http://purl.org/htp#HiTOP-T007eM -->

    <owl:Class rdf:about="http://purl.org/htp#HiTOP-T007eM">
        <rdfs:subClassOf rdf:resource="http://purl.org/htp#HiTOP-O002sP"/>
        <obo:iaoIAO_0000115 xml:lang="en">
            Anxiousness =def. an Internalizing which is characterized by a tendency to experience anxiety, nervousness, or unease, 
            often in response to stress or uncertainty, leading to heightened arousal or worry about future events.
        </obo:iaoIAO_0000115>
    </owl:Class>
    


    <!-- http://purl.org/htp#HiTOP-T008mD -->

    <owl:Class rdf:about="http://purl.org/htp#HiTOP-T008mD">
        <rdfs:subClassOf rdf:resource="http://purl.org/htp#HiTOP-O002sP"/>
        <obo:iaoIAO_0000115 xml:lang="en">
            Emotional Lability =def. an Internalizing which is characterized by rapid and intense emotional changes, often leading 
            to unpredictable shifts in mood, ranging from euphoria to sadness, with difficulty in regulating emotional responses.
        </obo:iaoIAO_0000115>
    </owl:Class>
    


    <!-- http://purl.org/htp#HiTOP-T0094I -->

    <owl:Class rdf:about="http://purl.org/htp#HiTOP-T0094I">
        <rdfs:subClassOf rdf:resource="http://purl.org/htp#HiTOP-O002sP"/>
        <obo:iaoIAO_0000115 xml:lang="en">
            Hostility =def. an Internalizing which is characterized by a tendency toward aggression, antagonism, or ill will 
            towards others, often accompanied by a deep-seated mistrust or negative attitudes, leading to interpersonal conflict.
        </obo:iaoIAO_0000115>
    </owl:Class>
    


    <!-- http://purl.org/htp#HiTOP-T00AZ -->

    <owl:Class rdf:about="http://purl.org/htp#HiTOP-T00AZ">
        <rdfs:subClassOf rdf:resource="http://purl.org/htp#HiTOP-O002sP"/>
        <obo:iaoIAO_0000115 xml:lang="en">
            Perseveration =def. an Internalizing which is characterized by the repetition of a particular response or 
            behavior despite the absence or cessation of a stimulus, often resulting in difficulty shifting attention or 
            adapting to changing situations.
        </obo:iaoIAO_0000115>
    </owl:Class>
    


    <!-- http://purl.org/htp#HiTOP-T00BXK -->

    <owl:Class rdf:about="http://purl.org/htp#HiTOP-T00BXK">
        <rdfs:subClassOf rdf:resource="http://purl.org/htp#HiTOP-O002sP"/>
        <obo:iaoIAO_0000115 xml:lang="en">
            (low) Restricted Affectivity =def. an Internalizing which is characterized by limited or constricted emotional expression, 
            often leading to a diminished range of emotional experiences or difficulty in expressing emotions in social or 
            interpersonal contexts.
        </obo:iaoIAO_0000115>
    </owl:Class>
    


    <!-- http://purl.org/htp#HiTOP-T00Cgy -->

    <owl:Class rdf:about="http://purl.org/htp#HiTOP-T00Cgy">
        <rdfs:subClassOf rdf:resource="http://purl.org/htp#HiTOP-O002sP"/>
        <obo:iaoIAO_0000115 xml:lang="en">
            Separation Insecurity =def. an Internalizing which is characterized by anxiety and insecurity in response to 
            separation from significant others, often leading to clinginess, fear of abandonment, and difficulty coping with 
            distance or changes in relationships.
        </obo:iaoIAO_0000115>
    </owl:Class>
    


    <!-- http://purl.org/htp#HiTOP-T00D42 -->

    <owl:Class rdf:about="http://purl.org/htp#HiTOP-T00D42">
        <rdfs:subClassOf rdf:resource="http://purl.org/htp#HiTOP-O002sP"/>
        <obo:iaoIAO_0000115 xml:lang="en">
            Submissiveness =def. an Internalizing which is characterized by a tendency to submit to others and avoid asserting oneself, 
            often resulting in passive behavior, difficulty in standing up for oneself, and a tendency to defer to the wishes or 
            authority of others.
        </obo:iaoIAO_0000115>
    </owl:Class>
    


    <!-- http://purl.org/htp#HiTOP-T00Eht -->

    <owl:Class rdf:about="http://purl.org/htp#HiTOP-T00Eht">
        <rdfs:subClassOf rdf:resource="http://purl.org/htp#HiTOP-O002sP"/>
        <obo:iaoIAO_0000115 xml:lang="en">
            Identity Problems =def. an Internalizing which is characterized by difficulties in forming or maintaining a stable sense of 
            self, often resulting in confusion about one's values, goals, or role in life, and leading to instability in 
            personal identity or self-concept.
        </obo:iaoIAO_0000115>
    </owl:Class>
    


    <!-- http://purl.org/htp#HiTOP-T00Fe0 -->

    <owl:Class rdf:about="http://purl.org/htp#HiTOP-T00Fe0">
        <rdfs:subClassOf rdf:resource="http://purl.org/htp#HiTOP-O002sP"/>
        <obo:iaoIAO_0000115 xml:lang="en">
            Negative Relationships =def. an Internalizing which is characterized by relationships that contribute to stress, 
            conflict, or emotional harm, often undermining well-being, personal growth, and the ability to form positive, 
            supportive connections with others.
        </obo:iaoIAO_0000115>
    </owl:Class>
    


    <!-- http://purl.org/htp#HiTOP-T00G3d -->

    <owl:Class rdf:about="http://purl.org/htp#HiTOP-T00G3d">
        <rdfs:subClassOf rdf:resource="http://purl.org/htp#HiTOP-O002sP"/>
        <obo:iaoIAO_0000115 xml:lang="en">
            Fragility =def. an Internalizing which is characterized by a lack of resilience and a tendency to be easily hurt or 
            affected by stress, often leading to emotional instability or difficulty coping with adversity.
        </obo:iaoIAO_0000115>
    </owl:Class>
    


    <!-- http://purl.org/htp#HiTOP-T00HCy -->

    <owl:Class rdf:about="http://purl.org/htp#HiTOP-T00HCy">
        <rdfs:subClassOf rdf:resource="http://purl.org/htp#HiTOP-O002sP"/>
        <obo:iaoIAO_0000115 xml:lang="en">
            Ineptitude =def. an Internalizing which is characterized by a lack of skill, competence, or ability in performing tasks 
            or handling situations, often resulting in difficulties in achieving goals or completing responsibilities.
        </obo:iaoIAO_0000115>
    </owl:Class>
    


    <!-- http://purl.org/htp#HiTOP-T00IAT -->

    <owl:Class rdf:about="http://purl.org/htp#HiTOP-T00IAT">
        <rdfs:subClassOf rdf:resource="http://purl.org/htp#HiTOP-O002sP"/>
        <obo:iaoIAO_0000115 xml:lang="en">
            (low) Invulnerability =def. an Internalizing which is characterized by a perception of being immune to harm or 
            negative effects, often leading to risky behavior, overconfidence, or a lack of consideration for potential consequences.
        </obo:iaoIAO_0000115>
    </owl:Class>
    


    <!-- http://purl.org/htp#HiTOP-T00ua9 -->

    <owl:Class rdf:about="http://purl.org/htp#HiTOP-T00ua9">
        <rdfs:subClassOf rdf:resource="http://purl.org/htp#HiTOP-O002sP"/>
        <obo:iaoIAO_0000115 xml:lang="en">
            Eccentricity =def. a Thought Disorder which is characterized by unconventional or peculiar behavior, 
            including odd mannerisms, unusual beliefs, or idiosyncratic ways of interacting with others.
        </obo:iaoIAO_0000115>
    </owl:Class>
    


    <!-- http://purl.org/htp#HiTOP-T00vjR -->

    <owl:Class rdf:about="http://purl.org/htp#HiTOP-T00vjR">
        <rdfs:subClassOf rdf:resource="http://purl.org/htp#HiTOP-O002sP"/>
        <obo:iaoIAO_0000115 xml:lang="en">
            Cognitive Perceptual Dysregulation =def. a Thought Disorder which is characterized by disturbances in cognition and 
            perception, including unusual beliefs, perceptual aberrations, and difficulties distinguishing internal thoughts 
            from external reality.
        </obo:iaoIAO_0000115>
    </owl:Class>
    


    <!-- http://purl.org/htp#HiTOP-T00wk6 -->

    <owl:Class rdf:about="http://purl.org/htp#HiTOP-T00wk6">
        <rdfs:subClassOf rdf:resource="http://purl.org/htp#HiTOP-O002sP"/>
        <obo:iaoIAO_0000115 xml:lang="en">
            Unusual Beliefs and Experiences =def. a Thought Disorder which is characterized by the presence of atypical beliefs 
            and perceptual experiences, such as magical thinking, perceptual distortions, or ideas of reference, that deviate 
            from cultural norms.
        </obo:iaoIAO_0000115>
    </owl:Class>
    


    <!-- http://purl.org/htp#HiTOP-T00xLn -->

    <owl:Class rdf:about="http://purl.org/htp#HiTOP-T00xLn">
        <rdfs:subClassOf rdf:resource="http://purl.org/htp#HiTOP-O002sP"/>
        <obo:iaoIAO_0000115 xml:lang="en">
            Fantasy Proneness =def. a Thought Disorder which is characterized by a tendency to engage in vivid and complex 
            fantasies, often involving imaginative immersion, daydreaming, or blurred boundaries between imagination and reality.
        </obo:iaoIAO_0000115>
    </owl:Class>
    


    <!-- http://purl.org/htp#HiTOP-T00yfU -->

    <owl:Class rdf:about="http://purl.org/htp#HiTOP-T00yfU">
        <rdfs:subClassOf rdf:resource="http://purl.org/htp#HiTOP-O002sP"/>
        <obo:iaoIAO_0000115 xml:lang="en">
            Depressivity =def. a Detachment which is characterized by persistent feelings of sadness, hopelessness, and 
            emotional pain, often accompanied by a diminished interest in life and a negative view of the self.
        </obo:iaoIAO_0000115>
    </owl:Class>
    


    <!-- http://purl.org/htp#HiTOP-T00zDk -->

    <owl:Class rdf:about="http://purl.org/htp#HiTOP-T00zDk">
        <rdfs:subClassOf rdf:resource="http://purl.org/htp#HiTOP-O002sP"/>
        <obo:iaoIAO_0000115 xml:lang="en">
            Intimacy Avoidance =def. a Detachment which is characterized by a tendency to avoid close relationships and 
            emotional intimacy, often due to discomfort with closeness, fear of vulnerability, or preference for emotional distance.
        </obo:iaoIAO_0000115>
    </owl:Class>
    


    <!-- http://purl.org/htp#HiTOP-T010c6 -->

    <owl:Class rdf:about="http://purl.org/htp#HiTOP-T010c6">
        <rdfs:subClassOf rdf:resource="http://purl.org/htp#HiTOP-O002sP"/>
        <obo:iaoIAO_0000115 xml:lang="en">
            Suspiciousness =def. a Detachment which is characterized by a tendency to be distrustful and suspicious of others, 
            often involving beliefs that others have harmful intentions or cannot be relied upon.
        </obo:iaoIAO_0000115>
    </owl:Class>
    


    <!-- http://purl.org/htp#HiTOP-T011K6 -->

    <owl:Class rdf:about="http://purl.org/htp#HiTOP-T011K6">
        <rdfs:subClassOf rdf:resource="http://purl.org/htp#HiTOP-O002sP"/>
        <obo:iaoIAO_0000115 xml:lang="en">
            Withdrawal =def. a Detachment which is characterized by a tendency to retreat from social interactions and avoid 
            engagement with others, often reflecting discomfort with social closeness or reduced motivation for 
            interpersonal connection.
        </obo:iaoIAO_0000115>
    </owl:Class>
    


    <!-- http://purl.org/htp#HiTOP-T012QL -->

    <owl:Class rdf:about="http://purl.org/htp#HiTOP-T012QL">
        <rdfs:subClassOf rdf:resource="http://purl.org/htp#HiTOP-O002sP"/>
        <obo:iaoIAO_0000115 xml:lang="en">
            Interpersonal Passivity =def. a Detachment which is characterized by a lack of initiative or assertiveness in 
            social interactions, often manifesting as submissiveness, indecision, or reluctance to express personal needs 
            or preferences.
        </obo:iaoIAO_0000115>
    </owl:Class>
    


    <!-- http://purl.org/htp#HiTOP-T013F1 -->

    <owl:Class rdf:about="http://purl.org/htp#HiTOP-T013F1">
        <rdfs:subClassOf rdf:resource="http://purl.org/htp#HiTOP-O002sP"/>
        <obo:iaoIAO_0000115 xml:lang="en">
            Disaffiliativeness =def. a Detachment which is characterized by a lack of interest in forming or maintaining 
            social bonds, often reflecting indifference toward closeness, companionship, or interpersonal connection.
        </obo:iaoIAO_0000115>
    </owl:Class>
    


    <!-- http://purl.org/htp#HiTOP-T014BA -->

    <owl:Class rdf:about="http://purl.org/htp#HiTOP-T014BA">
        <rdfs:subClassOf rdf:resource="http://purl.org/htp#HiTOP-O002sP"/>
        <obo:iaoIAO_0000115 xml:lang="en">
            (low) Attention Seeking =def. a Detachment which is characterized by a reduced or absent desire to attract and hold 
            the attention of others, often reflecting low social expressiveness or a preference for remaining unnoticed in 
            social settings.
        </obo:iaoIAO_0000115>
    </owl:Class>
    


    <!-- http://purl.org/htp#HiTOP-T015o8 -->

    <owl:Class rdf:about="http://purl.org/htp#HiTOP-T015o8">
        <rdfs:subClassOf rdf:resource="http://purl.org/htp#HiTOP-O002sP"/>
        <obo:iaoIAO_0000115 xml:lang="en">
            Problematic Impulsivity =def. a Disinhibited Externalizing which is characterized by difficulty in controlling 
            impulsive behaviors, often resulting in actions that lead to negative consequences for oneself or others.
        </obo:iaoIAO_0000115>
    </owl:Class>
    


    <!-- http://purl.org/htp#HiTOP-T016k0 -->

    <owl:Class rdf:about="http://purl.org/htp#HiTOP-T016k0">
        <rdfs:subClassOf rdf:resource="http://purl.org/htp#HiTOP-O002sP"/>
        <obo:iaoIAO_0000115 xml:lang="en">
            Irresponsibility =def. a Disinhibited Externalizing which is characterized by a lack of regard for the consequences 
            of one’s actions, often leading to reckless, careless, or socially inappropriate behaviors.
        </obo:iaoIAO_0000115>
    </owl:Class>
    


    <!-- http://purl.org/htp#HiTOP-T0177S -->

    <owl:Class rdf:about="http://purl.org/htp#HiTOP-T0177S">
        <rdfs:subClassOf rdf:resource="http://purl.org/htp#HiTOP-O002sP"/>
        <obo:iaoIAO_0000115 xml:lang="en">
            Theft =def. a Disinhibited Externalizing which is characterized by a tendency to steal or engage in dishonest 
            acquisition of property, often driven by impulsivity, disregard for social norms, or a lack of remorse.
        </obo:iaoIAO_0000115>
    </owl:Class>
    


    <!-- http://purl.org/htp#HiTOP-T018ir -->

    <owl:Class rdf:about="http://purl.org/htp#HiTOP-T018ir">
        <rdfs:subClassOf rdf:resource="http://purl.org/htp#HiTOP-O002sP"/>
        <obo:iaoIAO_0000115 xml:lang="en">
            Distractibility =def. a Disinhibited Externalizing which is characterized by an inability to maintain focus, 
            leading to frequent shifts in attention, impulsive responses to external stimuli, and difficulty completing tasks.
        </obo:iaoIAO_0000115>
    </owl:Class>
    


    <!-- http://purl.org/htp#HiTOP-T019Cj -->

    <owl:Class rdf:about="http://purl.org/htp#HiTOP-T019Cj">
        <rdfs:subClassOf rdf:resource="http://purl.org/htp#HiTOP-O002sP"/>
        <obo:iaoIAO_0000115 xml:lang="en">
            Risk Taking =def. a Disinhibited Externalizing which is characterized by engaging in behaviors that involve 
            significant risk, often without regard for potential negative outcomes or consequences, driven by a desire 
            for stimulation or thrill-seeking.
        </obo:iaoIAO_0000115>
    </owl:Class>
    


    <!-- http://purl.org/htp#HiTOP-T01A5i -->

    <owl:Class rdf:about="http://purl.org/htp#HiTOP-T01A5i">
        <rdfs:subClassOf rdf:resource="http://purl.org/htp#HiTOP-O002sP"/>
        <obo:iaoIAO_0000115 xml:lang="en">
            (low) Rigid Perfectionism =def. a Disinhibited Externalizing which is characterized by an excessive and inflexible 
            striving for perfection and high standards, often leading to self-criticism, stress, and difficulty adapting 
            to mistakes or setbacks.
        </obo:iaoIAO_0000115>
    </owl:Class>
    


    <!-- http://purl.org/htp#HiTOP-T01BfQ -->

    <owl:Class rdf:about="http://purl.org/htp#HiTOP-T01BfQ">
        <rdfs:subClassOf rdf:resource="http://purl.org/htp#HiTOP-O002sP"/>
        <obo:iaoIAO_0000115 xml:lang="en">
            (low) Ruminative Deliberation =def. a Disinhibited Externalizing which is characterized by excessive and repetitive 
            thinking about potential decisions and their outcomes, often leading to indecision, prolonged deliberation, and stress.
        </obo:iaoIAO_0000115>
    </owl:Class>
    


    <!-- http://purl.org/htp#HiTOP-T01C1W -->

    <owl:Class rdf:about="http://purl.org/htp#HiTOP-T01C1W">
        <rdfs:subClassOf rdf:resource="http://purl.org/htp#HiTOP-O002sP"/>
        <obo:iaoIAO_0000115 xml:lang="en">
            (low) Workaholism =def. a Disinhibited Externalizing which is characterized by an excessive and compulsive commitment 
            to work, often at the expense of personal well-being, relationships, and leisure time, leading to stress and burnout.
        </obo:iaoIAO_0000115>
    </owl:Class>
    


    <!-- http://purl.org/htp#HiTOP-T01Neb -->

    <owl:Class rdf:about="http://purl.org/htp#HiTOP-T01Neb">
        <rdfs:subClassOf rdf:resource="http://purl.org/htp#HiTOP-O002sP"/>
        <obo:iaoIAO_0000115 xml:lang="en">
            Impatient Urgency =def. an Antisocial Behavior which is characterized by a lack of patience and a tendency to act 
            impulsively in urgent situations, often leading to rash decisions and behaviors without consideration for the 
            consequences.
        </obo:iaoIAO_0000115>
    </owl:Class>
    


    <!-- http://purl.org/htp#HiTOP-T01OY2 -->

    <owl:Class rdf:about="http://purl.org/htp#HiTOP-T01OY2">
        <rdfs:subClassOf rdf:resource="http://purl.org/htp#HiTOP-O002sP"/>
        <obo:iaoIAO_0000115 xml:lang="en">
            (low) Planful Control =def. an Antisocial Behavior which is characterized by a poor ability to plan and execute 
            tasks effectively, often resulting in impulsive actions, disorganization, and an inability to meet goals 
            or manage responsibilities.
        </obo:iaoIAO_0000115>
    </owl:Class>
    


    <!-- http://purl.org/htp#HiTOP-T01PMW -->

    <owl:Class rdf:about="http://purl.org/htp#HiTOP-T01PMW">
        <rdfs:subClassOf rdf:resource="http://purl.org/htp#HiTOP-O002sP"/>
        <obo:iaoIAO_0000115 xml:lang="en">
            (low) Dependability =def. an Antisocial Behavior which is characterized by a lack of reliability and consistency 
            in fulfilling obligations, often resulting in failure to meet commitments or responsibilities, and 
            causing disruptions in personal or professional relationships.
        </obo:iaoIAO_0000115>
    </owl:Class>
    


    <!-- http://purl.org/htp#HiTOP-T01QNN -->

    <owl:Class rdf:about="http://purl.org/htp#HiTOP-T01QNN">
        <rdfs:subClassOf rdf:resource="http://purl.org/htp#HiTOP-O002sP"/>
        <obo:iaoIAO_0000115 xml:lang="en">
            Alienation =def. an Antisocial Behavior which is characterized by a sense of estrangement or detachment from others, 
            often leading to feelings of social isolation, loneliness, and a lack of connection to social groups or 
            society at large.
        </obo:iaoIAO_0000115>
    </owl:Class>
    


    <!-- http://purl.org/htp#HiTOP-T01RYG -->

    <owl:Class rdf:about="http://purl.org/htp#HiTOP-T01RYG">
        <rdfs:subClassOf rdf:resource="http://purl.org/htp#HiTOP-O002sP"/>
        <obo:iaoIAO_0000115 xml:lang="en">
            Boredom Proneness =def. an Antisocial Behavior which is characterized by a tendency to experience boredom frequently 
            and easily, often leading to restlessness, dissatisfaction, and a search for novel or stimulating experiences.
        </obo:iaoIAO_0000115>
    </owl:Class>
    


    <!-- http://purl.org/htp#HiTOP-T01SYW -->

    <owl:Class rdf:about="http://purl.org/htp#HiTOP-T01SYW">
        <rdfs:subClassOf rdf:resource="http://purl.org/htp#HiTOP-O002sP"/>
        <obo:iaoIAO_0000115 xml:lang="en">
            Blame Externalization =def. an Antisocial Behavior which is characterized by a tendency to attribute failures or 
            problems to external factors, such as other people, circumstances, or societal influences, rather than 
            recognizing internal causes or personal responsibility.
        </obo:iaoIAO_0000115>
    </owl:Class>
    


    <!-- http://purl.org/htp#HiTOP-T01T3u -->

    <owl:Class rdf:about="http://purl.org/htp#HiTOP-T01T3u">
        <rdfs:subClassOf rdf:resource="http://purl.org/htp#HiTOP-O002sP"/>
        <obo:iaoIAO_0000115 xml:lang="en">
            (low) Honesty =def. an Antisocial Behavior which is characterized by a tendency to be deceitful or untruthful, 
            often involving the manipulation of others or a disregard for truthfulness in social interactions.
        </obo:iaoIAO_0000115>
    </owl:Class>
    


    <!-- http://purl.org/htp#HiTOP-T01UGN -->

    <owl:Class rdf:about="http://purl.org/htp#HiTOP-T01UGN">
        <rdfs:subClassOf rdf:resource="http://purl.org/htp#HiTOP-O002sP"/>
        <obo:iaoIAO_0000115 xml:lang="en">
            Rebelliousness =def. an Antisocial Behavior which is characterized by resistance to authority, rules, and 
            societal norms, often manifested through defiance, disobedience, or challenging established systems or conventions.
        </obo:iaoIAO_0000115>
    </owl:Class>
    


    <!-- http://purl.org/htp#HiTOP-T01VXq -->

    <owl:Class rdf:about="http://purl.org/htp#HiTOP-T01VXq">
        <rdfs:subClassOf rdf:resource="http://purl.org/htp#HiTOP-O002sP"/>
        <obo:iaoIAO_0000115 xml:lang="en">
            (low) Empathy =def. an Antisocial Behavior which is characterized by a reduced ability to understand and 
            share the feelings of others, often leading to emotional detachment, indifference, or difficulty in 
            forming meaningful interpersonal connections.
        </obo:iaoIAO_0000115>
    </owl:Class>
    


    <!-- http://purl.org/htp#HiTOP-T01W1E -->

    <owl:Class rdf:about="http://purl.org/htp#HiTOP-T01W1E">
        <rdfs:subClassOf rdf:resource="http://purl.org/htp#HiTOP-O002sP"/>
        <obo:iaoIAO_0000115 xml:lang="en">
            Excitement Seeking =def. an Antisocial Behavior which is characterized by a desire for new, thrilling, 
            or risky experiences, often driving individuals to engage in activities that provide immediate gratification 
            or stimulation, regardless of potential consequences.
        </obo:iaoIAO_0000115>
    </owl:Class>
    


    <!-- http://purl.org/htp#HiTOP-T01XQi -->

    <owl:Class rdf:about="http://purl.org/htp#HiTOP-T01XQi">
        <rdfs:subClassOf rdf:resource="http://purl.org/htp#HiTOP-O002sP"/>
        <obo:iaoIAO_0000115 xml:lang="en">
            Attention Seeking =def. an Antagonistic Externalizing which is characterized by a constant need for validation 
            or recognition, often leading to behaviors aimed at drawing focus from others, typically through exaggerated actions, 
            statements, or displays.
        </obo:iaoIAO_0000115>
    </owl:Class>
    


    <!-- http://purl.org/htp#HiTOP-T01Y7w -->

    <owl:Class rdf:about="http://purl.org/htp#HiTOP-T01Y7w">
        <rdfs:subClassOf rdf:resource="http://purl.org/htp#HiTOP-O002sP"/>
        <obo:iaoIAO_0000115 xml:lang="en">
            Callousness =def. an Antagonistic Externalizing which is characterized by a lack of empathy and 
            a tendency to be emotionally cold or indifferent to others, often resulting in a disregard for the feelings 
            or well-being of others.
        </obo:iaoIAO_0000115>
    </owl:Class>
    


    <!-- http://purl.org/htp#HiTOP-T01Ziz -->

    <owl:Class rdf:about="http://purl.org/htp#HiTOP-T01Ziz">
        <rdfs:subClassOf rdf:resource="http://purl.org/htp#HiTOP-O002sP"/>
        <obo:iaoIAO_0000115 xml:lang="en">
            Deceitfulness =def. an Antagonistic Externalizing which is characterized by a tendency to lie, cheat, 
            or deceive others, often for personal gain, manipulation, or to avoid negative consequences.
        </obo:iaoIAO_0000115>
    </owl:Class>
    


    <!-- http://purl.org/htp#HiTOP-T01a7u -->

    <owl:Class rdf:about="http://purl.org/htp#HiTOP-T01a7u">
        <rdfs:subClassOf rdf:resource="http://purl.org/htp#HiTOP-O002sP"/>
        <obo:iaoIAO_0000115 xml:lang="en">
            Grandiosity =def. an Antagonistic Externalizing which is characterized by an exaggerated sense of one’s own importance, 
            abilities, or achievements, often accompanied by a lack of consideration for others and a belief in one's superiority 
            or entitlement.
        </obo:iaoIAO_0000115>
    </owl:Class>
    


    <!-- http://purl.org/htp#HiTOP-T01bz7 -->

    <owl:Class rdf:about="http://purl.org/htp#HiTOP-T01bz7">
        <rdfs:subClassOf rdf:resource="http://purl.org/htp#HiTOP-O002sP"/>
        <obo:iaoIAO_0000115 xml:lang="en">
            Manipulativeness =def. an Antagonistic Externalizing which is characterized by a tendency to control or 
            influence others for personal gain, often in a devious or underhanded manner, without regard for others' well-being or 
            autonomy.
        </obo:iaoIAO_0000115>
    </owl:Class>
    


    <!-- http://purl.org/htp#HiTOP-T01cX5 -->

    <owl:Class rdf:about="http://purl.org/htp#HiTOP-T01cX5">
        <rdfs:subClassOf rdf:resource="http://purl.org/htp#HiTOP-O002sP"/>
        <obo:iaoIAO_0000115 xml:lang="en">
            Rudeness =def. an Antagonistic Externalizing which is characterized by a lack of manners or 
            respect in social interactions, often involving offensive or inappropriate behaviors that disregard social norms 
            and conventions.
        </obo:iaoIAO_0000115>
    </owl:Class>
    


    <!-- http://purl.org/htp#HiTOP-T01d9I -->

    <owl:Class rdf:about="http://purl.org/htp#HiTOP-T01d9I">
        <rdfs:subClassOf rdf:resource="http://purl.org/htp#HiTOP-O002sP"/>
        <obo:iaoIAO_0000115 xml:lang="en">
            Egocentricity =def. an Antagonistic Externalizing which is characterized by an excessive focus on oneself 
            and one’s own needs and desires, often leading to a lack of consideration for others and a diminished capacity 
            for empathy or understanding of different perspectives.
        </obo:iaoIAO_0000115>
    </owl:Class>
    


    <!-- http://purl.org/htp#HiTOP-T01eG6 -->

    <owl:Class rdf:about="http://purl.org/htp#HiTOP-T01eG6">
        <rdfs:subClassOf rdf:resource="http://purl.org/htp#HiTOP-O002sP"/>
        <obo:iaoIAO_0000115 xml:lang="en">
            Dominance =def. an Antagonistic Externalizing which is characterized by a desire to control or lead others, 
            often displaying assertiveness, power, and a tendency to assert one's will over others in social or 
            organizational contexts.
        </obo:iaoIAO_0000115>
    </owl:Class>
    


    <!-- http://purl.org/htp#HiTOP-T01fc8 -->

    <owl:Class rdf:about="http://purl.org/htp#HiTOP-T01fc8">
        <rdfs:subClassOf rdf:resource="http://purl.org/htp#HiTOP-O002sP"/>
        <obo:iaoIAO_0000115 xml:lang="en">
            Flirtatiousness =def. an Antagonistic Externalizing which is characterized by behavior that seeks to attract 
            romantic or sexual interest from others through playful, suggestive, or provocative means, often involving charm 
            or manipulation.
        </obo:iaoIAO_0000115>
    </owl:Class>
    


    <!-- http://purl.org/htp#HiTOP-T01gKP -->

    <owl:Class rdf:about="http://purl.org/htp#HiTOP-T01gKP">
        <rdfs:subClassOf rdf:resource="http://purl.org/htp#HiTOP-O002sP"/>
        <obo:iaoIAO_0000115 xml:lang="en">
            (low) Timorousness =def. an Antagonistic Externalizing which is characterized by a tendency to be fearful 
            or lacking in confidence, often leading to shyness, hesitation, or avoidance of social interactions and 
            opportunities due to fear of judgment or failure.
        </obo:iaoIAO_0000115>
    </owl:Class>
    


    <!-- http://purl.org/htp#HiTOP-U0012Y -->

    <owl:Class rdf:about="http://purl.org/htp#HiTOP-U0012Y">
        <rdfs:subClassOf rdf:resource="http://purl.org/htp#HiTOP-O002sP"/>
        <obo:iaoIAO_0000115 xml:lang="en">
            Sexual Problems =def. an Internalizing which is characterized by difficulties and dysfunctions related
            to sexual health and behavior, reflecting internal psychological distress that manifests in sexual functioning.
        </obo:iaoIAO_0000115>
        <rdfs:comment xml:lang="en">
            Sexual Problems encompass difficulties and dysfunctions related to sexual health and behavior.
        </rdfs:comment>
        <rdfs:label xml:lang="en">Sexual Problems</rdfs:label>
        <skos:changeNote xml:lang="en">
            This subfactor is designed to be adaptable to future updates and expansions. 
            It allows for the incorporation of new elements or modifications to existing components as research advances and 
            our understanding of psychological phenomena evolves.
        </skos:changeNote>
    </owl:Class>
    


    <!-- http://purl.org/htp#HiTOP-U002SC -->

    <owl:Class rdf:about="http://purl.org/htp#HiTOP-U002SC">
        <rdfs:subClassOf rdf:resource="http://purl.org/htp#HiTOP-O002sP"/>
        <obo:iaoIAO_0000115 xml:lang="en">
            Eating Pathology =def. an Internalizing which is characterized by disordered eating behaviors and 
            maladaptive concerns related to body image, reflecting internal psychological distress expressed through eating 
            and self-perception.
        </obo:iaoIAO_0000115>
        <rdfs:comment xml:lang="en">
            Eating Pathology includes disorders and maladaptive behaviors related to eating and body image.
        </rdfs:comment>
        <rdfs:label xml:lang="en">Eating Pathology</rdfs:label>
        <skos:changeNote xml:lang="en">
            This subfactor is designed to be adaptable to future updates and expansions. 
            It allows for the incorporation of new elements or modifications to existing components as research advances and 
            our understanding of psychological phenomena evolves.
        </skos:changeNote>
    </owl:Class>
    


    <!-- http://purl.org/htp#HiTOP-U0036N -->

    <owl:Class rdf:about="http://purl.org/htp#HiTOP-U0036N">
        <rdfs:subClassOf rdf:resource="http://purl.org/htp#HiTOP-O002sP"/>
        <obo:iaoIAO_0000115 xml:lang="en">
            Fear =def. an Internalizing which is characterized by emotional responses to perceived threats or danger, 
            typically involving heightened arousal, avoidance behaviors, and anticipatory anxiety.
        </obo:iaoIAO_0000115>
        <rdfs:comment xml:lang="en">
            Fear refers to an emotional response to perceived threats or danger.
        </rdfs:comment>
        <rdfs:label xml:lang="en">Fear</rdfs:label>
        <skos:changeNote xml:lang="en">
            This subfactor is designed to be adaptable to future updates and expansions. 
            It allows for the incorporation of new elements or modifications to existing components as research advances and 
            our understanding of psychological phenomena evolves.
        </skos:changeNote>
    </owl:Class>
    


    <!-- http://purl.org/htp#HiTOP-U004dm -->

    <owl:Class rdf:about="http://purl.org/htp#HiTOP-U004dm">
        <rdfs:subClassOf rdf:resource="http://purl.org/htp#HiTOP-O002sP"/>
        <obo:iaoIAO_0000115 xml:lang="en">
            Distress =def. an Internalizing which is characterized by significant emotional suffering or discomfort, 
            often involving persistent negative affect such as sadness, hopelessness, or irritability.
        </obo:iaoIAO_0000115>
        <rdfs:comment xml:lang="en">
            Distress involves significant emotional suffering or discomfort.
        </rdfs:comment>
        <rdfs:label xml:lang="en">Distress</rdfs:label>
        <skos:changeNote xml:lang="en">
            This subfactor is designed to be adaptable to future updates and expansions. 
            It allows for the incorporation of new elements or modifications to existing components as research advances and 
            our understanding of psychological phenomena evolves.
        </skos:changeNote>
    </owl:Class>
    


    <!-- http://purl.org/htp#HiTOP-U005q -->

    <owl:Class rdf:about="http://purl.org/htp#HiTOP-U005q">
        <rdfs:subClassOf rdf:resource="http://purl.org/htp#HiTOP-O002sP"/>
        <obo:iaoIAO_0000115 xml:lang="en">
            Mania =def. an Internalizing and Thought Disorder which is characterized by elevated mood, 
            increased activity levels, and impulsive behavior, reflecting dysregulation in affective and cognitive functioning.
        </obo:iaoIAO_0000115>
        <rdfs:comment xml:lang="en">
            Mania is characterized by elevated mood, increased activity, and impulsive behavior.
        </rdfs:comment>
        <rdfs:label xml:lang="en">Mania</rdfs:label>
        <skos:changeNote xml:lang="en">
            This subfactor is designed to be adaptable to future updates and expansions. 
            It allows for the incorporation of new elements or modifications to existing components as research advances and 
            our understanding of psychological phenomena evolves.
        </skos:changeNote>
    </owl:Class>
    


    <!-- http://purl.org/htp#HiTOP-U0061L -->

    <owl:Class rdf:about="http://purl.org/htp#HiTOP-U0061L">
        <rdfs:subClassOf rdf:resource="http://purl.org/htp#HiTOP-O002sP"/>
        <obo:iaoIAO_0000115 xml:lang="en">
            Harmful Substance Abuse =def. a Disinhibited Externalizing which is characterized by excessive use of substances 
            that leads to significant harm or impairment in physical, psychological, or social functioning.
        </obo:iaoIAO_0000115>
        <rdfs:comment xml:lang="en">
            Harmful Substance Abuse refers to the excessive use of substances that causes significant harm or impairment.
        </rdfs:comment>
        <rdfs:label xml:lang="en">Harmful Substance Abuse</rdfs:label>
        <skos:changeNote xml:lang="en">
            This subfactor is designed to be adaptable to future updates and expansions. 
            It allows for the incorporation of new elements or modifications to existing components as research advances and 
            our understanding of psychological phenomena evolves.
        </skos:changeNote>
    </owl:Class>
    


    <!-- http://purl.org/htp#HiTOP-U007EJ -->

    <owl:Class rdf:about="http://purl.org/htp#HiTOP-U007EJ">
        <rdfs:subClassOf rdf:resource="http://purl.org/htp#HiTOP-O002sP"/>
        <obo:iaoIAO_0000115 xml:lang="en">
            Antisocial Behavior =def. a Disinhibited Externalizing and Antagonistic Externalizing which is characterized 
            by actions that violate societal norms and the rights of others, reflecting a combination of poor impulse control 
            and interpersonal antagonism.
        </obo:iaoIAO_0000115>
        <rdfs:comment xml:lang="en">
            Antisocial Behavior involves actions that violate societal norms and the rights of others.
        </rdfs:comment>
        <rdfs:label xml:lang="en">Antisocial Behavior</rdfs:label>
        <skos:changeNote xml:lang="en">
            This subfactor is designed to be adaptable to future updates and expansions. 
            It allows for the incorporation of new elements or modifications to existing components as research advances and 
            our understanding of psychological phenomena evolves.
        </skos:changeNote>
    </owl:Class>
    


    <!-- http://www.w3.org/1999/02/22-rdf-syntax-ns#DatatypeProperty -->

    <owl:Class rdf:about="http://www.w3.org/1999/02/22-rdf-syntax-ns#DatatypeProperty"/>
    


    <!-- http://www.w3.org/2002/07/owl#NamedIndividual -->

    <owl:Class rdf:about="http://www.w3.org/2002/07/owl#NamedIndividual"/>
    


    <!-- http://xmlns.com/foaf/0.1/Person -->

    <owl:Class rdf:about="http://xmlns.com/foaf/0.1/Person"/>
    


    <!-- 
    ///////////////////////////////////////////////////////////////////////////////////////
    //
    // Individuals
    //
    ///////////////////////////////////////////////////////////////////////////////////////
     -->

    


    <!-- http://purl.org/htp#HiTOP-C001qy -->

    <owl:NamedIndividual rdf:about="http://purl.org/htp#HiTOP-C001qy">
        <rdf:type rdf:resource="http://purl.org/htp#HiTOP-O002sP"/>
        <hasVersionID>1.0</hasVersionID>
    </owl:NamedIndividual>
    


    <!-- http://purl.org/htp#HiTOP-C00217 -->

    <owl:NamedIndividual rdf:about="http://purl.org/htp#HiTOP-C00217">
        <rdf:type rdf:resource="http://purl.org/htp#HiTOP-O002sP"/>
        <hasVersionID>1.0</hasVersionID>
    </owl:NamedIndividual>
    


    <!-- http://purl.org/htp#HiTOP-C0033z -->

    <owl:NamedIndividual rdf:about="http://purl.org/htp#HiTOP-C0033z">
        <rdf:type rdf:resource="http://purl.org/htp#HiTOP-O002sP"/>
        <hasVersionID>1.0</hasVersionID>
    </owl:NamedIndividual>
    


    <!-- http://purl.org/htp#HiTOP-C00416 -->

    <owl:NamedIndividual rdf:about="http://purl.org/htp#HiTOP-C00416">
        <rdf:type rdf:resource="http://purl.org/htp#HiTOP-O002sP"/>
        <hasVersionID>1.0</hasVersionID>
    </owl:NamedIndividual>
    


    <!-- http://purl.org/htp#HiTOP-C005Sv -->

    <owl:NamedIndividual rdf:about="http://purl.org/htp#HiTOP-C005Sv">
        <rdf:type rdf:resource="http://purl.org/htp#HiTOP-O002sP"/>
        <hasVersionID>1.0</hasVersionID>
    </owl:NamedIndividual>
    


    <!-- http://purl.org/htp#HiTOP-C006MD -->

    <owl:NamedIndividual rdf:about="http://purl.org/htp#HiTOP-C006MD">
        <rdf:type rdf:resource="http://purl.org/htp#HiTOP-O002sP"/>
        <hasVersionID>1.0</hasVersionID>
    </owl:NamedIndividual>
    


    <!-- http://purl.org/htp#HiTOP-C00JTU -->

    <owl:NamedIndividual rdf:about="http://purl.org/htp#HiTOP-C00JTU">
        <rdf:type rdf:resource="http://purl.org/htp#HiTOP-O002sP"/>
        <hasVersionID>1.0</hasVersionID>
    </owl:NamedIndividual>
    


    <!-- http://purl.org/htp#HiTOP-C00KL0 -->

    <owl:NamedIndividual rdf:about="http://purl.org/htp#HiTOP-C00KL0">
        <rdf:type rdf:resource="http://purl.org/htp#HiTOP-O002sP"/>
        <hasVersionID>1.0</hasVersionID>
    </owl:NamedIndividual>
    


    <!-- http://purl.org/htp#HiTOP-C00LqY -->

    <owl:NamedIndividual rdf:about="http://purl.org/htp#HiTOP-C00LqY">
        <rdf:type rdf:resource="http://purl.org/htp#HiTOP-O002sP"/>
        <hasVersionID>1.0</hasVersionID>
    </owl:NamedIndividual>
    


    <!-- http://purl.org/htp#HiTOP-C00Mpl -->

    <owl:NamedIndividual rdf:about="http://purl.org/htp#HiTOP-C00Mpl">
        <rdf:type rdf:resource="http://purl.org/htp#HiTOP-O002sP"/>
        <hasVersionID>1.0</hasVersionID>
    </owl:NamedIndividual>
    


    <!-- http://purl.org/htp#HiTOP-C00N4I -->

    <owl:NamedIndividual rdf:about="http://purl.org/htp#HiTOP-C00N4I">
        <rdf:type rdf:resource="http://purl.org/htp#HiTOP-O002sP"/>
        <hasVersionID>1.0</hasVersionID>
    </owl:NamedIndividual>
    


    <!-- http://purl.org/htp#HiTOP-C00OuR -->

    <owl:NamedIndividual rdf:about="http://purl.org/htp#HiTOP-C00OuR">
        <rdf:type rdf:resource="http://purl.org/htp#HiTOP-O002sP"/>
        <hasVersionID>1.0</hasVersionID>
    </owl:NamedIndividual>
    


    <!-- http://purl.org/htp#HiTOP-C00Pjp -->

    <owl:NamedIndividual rdf:about="http://purl.org/htp#HiTOP-C00Pjp">
        <rdf:type rdf:resource="http://purl.org/htp#HiTOP-O002sP"/>
        <hasVersionID>1.0</hasVersionID>
    </owl:NamedIndividual>
    


    <!-- http://purl.org/htp#HiTOP-C00Q1t -->

    <owl:NamedIndividual rdf:about="http://purl.org/htp#HiTOP-C00Q1t">
        <rdf:type rdf:resource="http://purl.org/htp#HiTOP-O002sP"/>
        <hasVersionID>1.0</hasVersionID>
    </owl:NamedIndividual>
    


    <!-- http://purl.org/htp#HiTOP-C00RGy -->

    <owl:NamedIndividual rdf:about="http://purl.org/htp#HiTOP-C00RGy">
        <rdf:type rdf:resource="http://purl.org/htp#HiTOP-O002sP"/>
        <hasVersionID>1.0</hasVersionID>
    </owl:NamedIndividual>
    


    <!-- http://purl.org/htp#HiTOP-C00S9m -->

    <owl:NamedIndividual rdf:about="http://purl.org/htp#HiTOP-C00S9m">
        <rdf:type rdf:resource="http://purl.org/htp#HiTOP-O002sP"/>
        <hasVersionID>1.0</hasVersionID>
    </owl:NamedIndividual>
    


    <!-- http://purl.org/htp#HiTOP-C00TgL -->

    <owl:NamedIndividual rdf:about="http://purl.org/htp#HiTOP-C00TgL">
        <rdf:type rdf:resource="http://purl.org/htp#HiTOP-O002sP"/>
        <hasVersionID>1.0</hasVersionID>
    </owl:NamedIndividual>
    


    <!-- http://purl.org/htp#HiTOP-C00Urw -->

    <owl:NamedIndividual rdf:about="http://purl.org/htp#HiTOP-C00Urw">
        <rdf:type rdf:resource="http://purl.org/htp#HiTOP-O002sP"/>
        <hasVersionID>1.0</hasVersionID>
    </owl:NamedIndividual>
    


    <!-- http://purl.org/htp#HiTOP-C00VHv -->

    <owl:NamedIndividual rdf:about="http://purl.org/htp#HiTOP-C00VHv">
        <rdf:type rdf:resource="http://purl.org/htp#HiTOP-O002sP"/>
        <hasVersionID>1.0</hasVersionID>
    </owl:NamedIndividual>
    


    <!-- http://purl.org/htp#HiTOP-C00WJc -->

    <owl:NamedIndividual rdf:about="http://purl.org/htp#HiTOP-C00WJc">
        <rdf:type rdf:resource="http://purl.org/htp#HiTOP-O002sP"/>
        <hasVersionID>1.0</hasVersionID>
    </owl:NamedIndividual>
    


    <!-- http://purl.org/htp#HiTOP-C00XyI -->

    <owl:NamedIndividual rdf:about="http://purl.org/htp#HiTOP-C00XyI">
        <rdf:type rdf:resource="http://purl.org/htp#HiTOP-O002sP"/>
        <hasVersionID>1.0</hasVersionID>
    </owl:NamedIndividual>
    


    <!-- http://purl.org/htp#HiTOP-C00Y8j -->

    <owl:NamedIndividual rdf:about="http://purl.org/htp#HiTOP-C00Y8j">
        <rdf:type rdf:resource="http://purl.org/htp#HiTOP-O002sP"/>
        <hasVersionID>1.0</hasVersionID>
    </owl:NamedIndividual>
    


    <!-- http://purl.org/htp#HiTOP-C00ZyP -->

    <owl:NamedIndividual rdf:about="http://purl.org/htp#HiTOP-C00ZyP">
        <rdf:type rdf:resource="http://purl.org/htp#HiTOP-O002sP"/>
        <hasVersionID>1.0</hasVersionID>
    </owl:NamedIndividual>
    


    <!-- http://purl.org/htp#HiTOP-C00aMF -->

    <owl:NamedIndividual rdf:about="http://purl.org/htp#HiTOP-C00aMF">
        <rdf:type rdf:resource="http://purl.org/htp#HiTOP-O002sP"/>
        <hasVersionID>1.0</hasVersionID>
    </owl:NamedIndividual>
    


    <!-- http://purl.org/htp#HiTOP-C00bEx -->

    <owl:NamedIndividual rdf:about="http://purl.org/htp#HiTOP-C00bEx">
        <rdf:type rdf:resource="http://purl.org/htp#HiTOP-O002sP"/>
        <hasVersionID>1.0</hasVersionID>
    </owl:NamedIndividual>
    


    <!-- http://purl.org/htp#HiTOP-C00cSn -->

    <owl:NamedIndividual rdf:about="http://purl.org/htp#HiTOP-C00cSn">
        <rdf:type rdf:resource="http://purl.org/htp#HiTOP-O002sP"/>
        <hasVersionID>1.0</hasVersionID>
    </owl:NamedIndividual>
    


    <!-- http://purl.org/htp#HiTOP-C00dc1 -->

    <owl:NamedIndividual rdf:about="http://purl.org/htp#HiTOP-C00dc1">
        <rdf:type rdf:resource="http://purl.org/htp#HiTOP-O002sP"/>
        <hasVersionID>1.0</hasVersionID>
    </owl:NamedIndividual>
    


    <!-- http://purl.org/htp#HiTOP-C00eL -->

    <owl:NamedIndividual rdf:about="http://purl.org/htp#HiTOP-C00eL">
        <rdf:type rdf:resource="http://purl.org/htp#HiTOP-O002sP"/>
        <hasVersionID>1.0</hasVersionID>
    </owl:NamedIndividual>
    


    <!-- http://purl.org/htp#HiTOP-C00fKQ -->

    <owl:NamedIndividual rdf:about="http://purl.org/htp#HiTOP-C00fKQ">
        <rdf:type rdf:resource="http://purl.org/htp#HiTOP-O002sP"/>
        <hasVersionID>1.0</hasVersionID>
    </owl:NamedIndividual>
    


    <!-- http://purl.org/htp#HiTOP-C00gvD -->

    <owl:NamedIndividual rdf:about="http://purl.org/htp#HiTOP-C00gvD">
        <rdf:type rdf:resource="http://purl.org/htp#HiTOP-O002sP"/>
        <hasVersionID>1.0</hasVersionID>
    </owl:NamedIndividual>
    


    <!-- http://purl.org/htp#HiTOP-C00hPJ -->

    <owl:NamedIndividual rdf:about="http://purl.org/htp#HiTOP-C00hPJ">
        <rdf:type rdf:resource="http://purl.org/htp#HiTOP-O002sP"/>
        <hasVersionID>1.0</hasVersionID>
    </owl:NamedIndividual>
    


    <!-- http://purl.org/htp#HiTOP-C00iAh -->

    <owl:NamedIndividual rdf:about="http://purl.org/htp#HiTOP-C00iAh">
        <rdf:type rdf:resource="http://purl.org/htp#HiTOP-O002sP"/>
        <hasVersionID>1.0</hasVersionID>
    </owl:NamedIndividual>
    


    <!-- http://purl.org/htp#HiTOP-C00jw5 -->

    <owl:NamedIndividual rdf:about="http://purl.org/htp#HiTOP-C00jw5">
        <rdf:type rdf:resource="http://purl.org/htp#HiTOP-O002sP"/>
        <hasVersionID>1.0</hasVersionID>
    </owl:NamedIndividual>
    


    <!-- http://purl.org/htp#HiTOP-C00kEN -->

    <owl:NamedIndividual rdf:about="http://purl.org/htp#HiTOP-C00kEN">
        <rdf:type rdf:resource="http://purl.org/htp#HiTOP-O002sP"/>
        <hasVersionID>1.0</hasVersionID>
    </owl:NamedIndividual>
    


    <!-- http://purl.org/htp#HiTOP-C00l5y -->

    <owl:NamedIndividual rdf:about="http://purl.org/htp#HiTOP-C00l5y">
        <rdf:type rdf:resource="http://purl.org/htp#HiTOP-O002sP"/>
        <hasVersionID>1.0</hasVersionID>
    </owl:NamedIndividual>
    


    <!-- http://purl.org/htp#HiTOP-C00mpe -->

    <owl:NamedIndividual rdf:about="http://purl.org/htp#HiTOP-C00mpe">
        <rdf:type rdf:resource="http://purl.org/htp#HiTOP-O002sP"/>
        <hasVersionID>1.0</hasVersionID>
    </owl:NamedIndividual>
    


    <!-- http://purl.org/htp#HiTOP-C00nyb -->

    <owl:NamedIndividual rdf:about="http://purl.org/htp#HiTOP-C00nyb">
        <rdf:type rdf:resource="http://purl.org/htp#HiTOP-O002sP"/>
        <hasVersionID>1.0</hasVersionID>
    </owl:NamedIndividual>
    


    <!-- http://purl.org/htp#HiTOP-C00oKM -->

    <owl:NamedIndividual rdf:about="http://purl.org/htp#HiTOP-C00oKM">
        <rdf:type rdf:resource="http://purl.org/htp#HiTOP-O002sP"/>
        <hasVersionID>1.0</hasVersionID>
    </owl:NamedIndividual>
    


    <!-- http://purl.org/htp#HiTOP-C00pnZ -->

    <owl:NamedIndividual rdf:about="http://purl.org/htp#HiTOP-C00pnZ">
        <rdf:type rdf:resource="http://purl.org/htp#HiTOP-O002sP"/>
        <hasVersionID>1.0</hasVersionID>
    </owl:NamedIndividual>
    


    <!-- http://purl.org/htp#HiTOP-C00qSD -->

    <owl:NamedIndividual rdf:about="http://purl.org/htp#HiTOP-C00qSD">
        <rdf:type rdf:resource="http://purl.org/htp#HiTOP-O002sP"/>
        <hasVersionID>1.0</hasVersionID>
    </owl:NamedIndividual>
    


    <!-- http://purl.org/htp#HiTOP-C00rnS -->

    <owl:NamedIndividual rdf:about="http://purl.org/htp#HiTOP-C00rnS">
        <rdf:type rdf:resource="http://purl.org/htp#HiTOP-O002sP"/>
        <hasVersionID>1.0</hasVersionID>
    </owl:NamedIndividual>
    


    <!-- http://purl.org/htp#HiTOP-C00sWr -->

    <owl:NamedIndividual rdf:about="http://purl.org/htp#HiTOP-C00sWr">
        <rdf:type rdf:resource="http://purl.org/htp#HiTOP-O002sP"/>
        <hasVersionID>1.0</hasVersionID>
    </owl:NamedIndividual>
    


    <!-- http://purl.org/htp#HiTOP-C00tUQ -->

    <owl:NamedIndividual rdf:about="http://purl.org/htp#HiTOP-C00tUQ">
        <rdf:type rdf:resource="http://purl.org/htp#HiTOP-O002sP"/>
        <hasVersionID>1.0</hasVersionID>
    </owl:NamedIndividual>
    


    <!-- http://purl.org/htp#HiTOP-C01DAb -->

    <owl:NamedIndividual rdf:about="http://purl.org/htp#HiTOP-C01DAb">
        <rdf:type rdf:resource="http://purl.org/htp#HiTOP-O002sP"/>
        <hasVersionID>1.0</hasVersionID>
    </owl:NamedIndividual>
    


    <!-- http://purl.org/htp#HiTOP-C01Elz -->

    <owl:NamedIndividual rdf:about="http://purl.org/htp#HiTOP-C01Elz">
        <rdf:type rdf:resource="http://purl.org/htp#HiTOP-O002sP"/>
        <hasVersionID>1.0</hasVersionID>
    </owl:NamedIndividual>
    


    <!-- http://purl.org/htp#HiTOP-C01FDy -->

    <owl:NamedIndividual rdf:about="http://purl.org/htp#HiTOP-C01FDy">
        <rdf:type rdf:resource="http://purl.org/htp#HiTOP-O002sP"/>
        <hasVersionID>1.0</hasVersionID>
    </owl:NamedIndividual>
    


    <!-- http://purl.org/htp#HiTOP-C01GEY -->

    <owl:NamedIndividual rdf:about="http://purl.org/htp#HiTOP-C01GEY">
        <rdf:type rdf:resource="http://purl.org/htp#HiTOP-O002sP"/>
        <hasVersionID>1.0</hasVersionID>
    </owl:NamedIndividual>
    


    <!-- http://purl.org/htp#HiTOP-C01HGq -->

    <owl:NamedIndividual rdf:about="http://purl.org/htp#HiTOP-C01HGq">
        <rdf:type rdf:resource="http://purl.org/htp#HiTOP-O002sP"/>
        <hasVersionID>1.0</hasVersionID>
    </owl:NamedIndividual>
    


    <!-- http://purl.org/htp#HiTOP-C01Ip4 -->

    <owl:NamedIndividual rdf:about="http://purl.org/htp#HiTOP-C01Ip4">
        <rdf:type rdf:resource="http://purl.org/htp#HiTOP-O002sP"/>
        <hasVersionID>1.0</hasVersionID>
    </owl:NamedIndividual>
    


    <!-- http://purl.org/htp#HiTOP-C01JH8 -->

    <owl:NamedIndividual rdf:about="http://purl.org/htp#HiTOP-C01JH8">
        <rdf:type rdf:resource="http://purl.org/htp#HiTOP-O002sP"/>
        <hasVersionID>1.0</hasVersionID>
    </owl:NamedIndividual>
    


    <!-- http://purl.org/htp#HiTOP-C01KXo -->

    <owl:NamedIndividual rdf:about="http://purl.org/htp#HiTOP-C01KXo">
        <rdf:type rdf:resource="http://purl.org/htp#HiTOP-O002sP"/>
        <hasVersionID>1.0</hasVersionID>
    </owl:NamedIndividual>
    


    <!-- http://purl.org/htp#HiTOP-C01LSp -->

    <owl:NamedIndividual rdf:about="http://purl.org/htp#HiTOP-C01LSp">
        <rdf:type rdf:resource="http://purl.org/htp#HiTOP-O002sP"/>
        <hasVersionID>1.0</hasVersionID>
    </owl:NamedIndividual>
    


    <!-- http://purl.org/htp#HiTOP-C01MjB -->

    <owl:NamedIndividual rdf:about="http://purl.org/htp#HiTOP-C01MjB">
        <rdf:type rdf:resource="http://purl.org/htp#HiTOP-O002sP"/>
        <hasVersionID>1.0</hasVersionID>
    </owl:NamedIndividual>
    


    <!-- http://purl.org/htp#HiTOP-T007eM -->

    <owl:NamedIndividual rdf:about="http://purl.org/htp#HiTOP-T007eM">
        <rdf:type rdf:resource="http://purl.org/htp#HiTOP-O002sP"/>
        <hasVersionID>1.0</hasVersionID>
    </owl:NamedIndividual>
    


    <!-- http://purl.org/htp#HiTOP-T008mD -->

    <owl:NamedIndividual rdf:about="http://purl.org/htp#HiTOP-T008mD">
        <rdf:type rdf:resource="http://purl.org/htp#HiTOP-O002sP"/>
        <hasVersionID>1.0</hasVersionID>
    </owl:NamedIndividual>
    


    <!-- http://purl.org/htp#HiTOP-T0094I -->

    <owl:NamedIndividual rdf:about="http://purl.org/htp#HiTOP-T0094I">
        <rdf:type rdf:resource="http://purl.org/htp#HiTOP-O002sP"/>
        <hasVersionID>1.0</hasVersionID>
    </owl:NamedIndividual>
    


    <!-- http://purl.org/htp#HiTOP-T00AZ -->

    <owl:NamedIndividual rdf:about="http://purl.org/htp#HiTOP-T00AZ">
        <rdf:type rdf:resource="http://purl.org/htp#HiTOP-O002sP"/>
        <hasVersionID>1.0</hasVersionID>
    </owl:NamedIndividual>
    


    <!-- http://purl.org/htp#HiTOP-T00BXK -->

    <owl:NamedIndividual rdf:about="http://purl.org/htp#HiTOP-T00BXK">
        <rdf:type rdf:resource="http://purl.org/htp#HiTOP-O002sP"/>
        <hasVersionID>1.0</hasVersionID>
    </owl:NamedIndividual>
    


    <!-- http://purl.org/htp#HiTOP-T00Cgy -->

    <owl:NamedIndividual rdf:about="http://purl.org/htp#HiTOP-T00Cgy">
        <rdf:type rdf:resource="http://purl.org/htp#HiTOP-O002sP"/>
        <hasVersionID>1.0</hasVersionID>
    </owl:NamedIndividual>
    


    <!-- http://purl.org/htp#HiTOP-T00D42 -->

    <owl:NamedIndividual rdf:about="http://purl.org/htp#HiTOP-T00D42">
        <rdf:type rdf:resource="http://purl.org/htp#HiTOP-O002sP"/>
        <hasVersionID>1.0</hasVersionID>
    </owl:NamedIndividual>
    


    <!-- http://purl.org/htp#HiTOP-T00Eht -->

    <owl:NamedIndividual rdf:about="http://purl.org/htp#HiTOP-T00Eht">
        <rdf:type rdf:resource="http://purl.org/htp#HiTOP-O002sP"/>
        <hasVersionID>1.0</hasVersionID>
    </owl:NamedIndividual>
    


    <!-- http://purl.org/htp#HiTOP-T00Fe0 -->

    <owl:NamedIndividual rdf:about="http://purl.org/htp#HiTOP-T00Fe0">
        <rdf:type rdf:resource="http://purl.org/htp#HiTOP-O002sP"/>
        <hasVersionID>1.0</hasVersionID>
    </owl:NamedIndividual>
    


    <!-- http://purl.org/htp#HiTOP-T00G3d -->

    <owl:NamedIndividual rdf:about="http://purl.org/htp#HiTOP-T00G3d">
        <rdf:type rdf:resource="http://purl.org/htp#HiTOP-O002sP"/>
        <hasVersionID>1.0</hasVersionID>
    </owl:NamedIndividual>
    


    <!-- http://purl.org/htp#HiTOP-T00HCy -->

    <owl:NamedIndividual rdf:about="http://purl.org/htp#HiTOP-T00HCy">
        <rdf:type rdf:resource="http://purl.org/htp#HiTOP-O002sP"/>
        <hasVersionID>1.0</hasVersionID>
    </owl:NamedIndividual>
    


    <!-- http://purl.org/htp#HiTOP-T00IAT -->

    <owl:NamedIndividual rdf:about="http://purl.org/htp#HiTOP-T00IAT">
        <rdf:type rdf:resource="http://purl.org/htp#HiTOP-O002sP"/>
        <hasVersionID>1.0</hasVersionID>
    </owl:NamedIndividual>
    


    <!-- http://purl.org/htp#HiTOP-T00ua9 -->

    <owl:NamedIndividual rdf:about="http://purl.org/htp#HiTOP-T00ua9">
        <rdf:type rdf:resource="http://purl.org/htp#HiTOP-O002sP"/>
        <hasVersionID>1.0</hasVersionID>
    </owl:NamedIndividual>
    


    <!-- http://purl.org/htp#HiTOP-T00vjR -->

    <owl:NamedIndividual rdf:about="http://purl.org/htp#HiTOP-T00vjR">
        <rdf:type rdf:resource="http://purl.org/htp#HiTOP-O002sP"/>
        <hasVersionID>1.0</hasVersionID>
    </owl:NamedIndividual>
    


    <!-- http://purl.org/htp#HiTOP-T00wk6 -->

    <owl:NamedIndividual rdf:about="http://purl.org/htp#HiTOP-T00wk6">
        <rdf:type rdf:resource="http://purl.org/htp#HiTOP-O002sP"/>
        <hasVersionID>1.0</hasVersionID>
    </owl:NamedIndividual>
    


    <!-- http://purl.org/htp#HiTOP-T00xLn -->

    <owl:NamedIndividual rdf:about="http://purl.org/htp#HiTOP-T00xLn">
        <rdf:type rdf:resource="http://purl.org/htp#HiTOP-O002sP"/>
        <hasVersionID>1.0</hasVersionID>
    </owl:NamedIndividual>
    


    <!-- http://purl.org/htp#HiTOP-T00yfU -->

    <owl:NamedIndividual rdf:about="http://purl.org/htp#HiTOP-T00yfU">
        <rdf:type rdf:resource="http://purl.org/htp#HiTOP-O002sP"/>
        <hasVersionID>1.0</hasVersionID>
    </owl:NamedIndividual>
    


    <!-- http://purl.org/htp#HiTOP-T00zDk -->

    <owl:NamedIndividual rdf:about="http://purl.org/htp#HiTOP-T00zDk">
        <rdf:type rdf:resource="http://purl.org/htp#HiTOP-O002sP"/>
        <hasVersionID>1.0</hasVersionID>
    </owl:NamedIndividual>
    


    <!-- http://purl.org/htp#HiTOP-T010c6 -->

    <owl:NamedIndividual rdf:about="http://purl.org/htp#HiTOP-T010c6">
        <rdf:type rdf:resource="http://purl.org/htp#HiTOP-O002sP"/>
        <hasVersionID>1.0</hasVersionID>
    </owl:NamedIndividual>
    


    <!-- http://purl.org/htp#HiTOP-T011K6 -->

    <owl:NamedIndividual rdf:about="http://purl.org/htp#HiTOP-T011K6">
        <rdf:type rdf:resource="http://purl.org/htp#HiTOP-O002sP"/>
        <hasVersionID>1.0</hasVersionID>
    </owl:NamedIndividual>
    


    <!-- http://purl.org/htp#HiTOP-T012QL -->

    <owl:NamedIndividual rdf:about="http://purl.org/htp#HiTOP-T012QL">
        <rdf:type rdf:resource="http://purl.org/htp#HiTOP-O002sP"/>
        <hasVersionID>1.0</hasVersionID>
    </owl:NamedIndividual>
    


    <!-- http://purl.org/htp#HiTOP-T013F1 -->

    <owl:NamedIndividual rdf:about="http://purl.org/htp#HiTOP-T013F1">
        <rdf:type rdf:resource="http://purl.org/htp#HiTOP-O002sP"/>
        <hasVersionID>1.0</hasVersionID>
    </owl:NamedIndividual>
    


    <!-- http://purl.org/htp#HiTOP-T014BA -->

    <owl:NamedIndividual rdf:about="http://purl.org/htp#HiTOP-T014BA">
        <rdf:type rdf:resource="http://purl.org/htp#HiTOP-O002sP"/>
        <hasVersionID>1.0</hasVersionID>
    </owl:NamedIndividual>
    


    <!-- http://purl.org/htp#HiTOP-T015o8 -->

    <owl:NamedIndividual rdf:about="http://purl.org/htp#HiTOP-T015o8">
        <rdf:type rdf:resource="http://purl.org/htp#HiTOP-O002sP"/>
        <hasVersionID>1.0</hasVersionID>
    </owl:NamedIndividual>
    


    <!-- http://purl.org/htp#HiTOP-T016k0 -->

    <owl:NamedIndividual rdf:about="http://purl.org/htp#HiTOP-T016k0">
        <rdf:type rdf:resource="http://purl.org/htp#HiTOP-O002sP"/>
        <hasVersionID>1.0</hasVersionID>
    </owl:NamedIndividual>
    


    <!-- http://purl.org/htp#HiTOP-T0177S -->

    <owl:NamedIndividual rdf:about="http://purl.org/htp#HiTOP-T0177S">
        <rdf:type rdf:resource="http://purl.org/htp#HiTOP-O002sP"/>
        <hasVersionID>1.0</hasVersionID>
    </owl:NamedIndividual>
    


    <!-- http://purl.org/htp#HiTOP-T018ir -->

    <owl:NamedIndividual rdf:about="http://purl.org/htp#HiTOP-T018ir">
        <rdf:type rdf:resource="http://purl.org/htp#HiTOP-O002sP"/>
        <hasVersionID>1.0</hasVersionID>
    </owl:NamedIndividual>
    


    <!-- http://purl.org/htp#HiTOP-T019Cj -->

    <owl:NamedIndividual rdf:about="http://purl.org/htp#HiTOP-T019Cj">
        <rdf:type rdf:resource="http://purl.org/htp#HiTOP-O002sP"/>
        <hasVersionID>1.0</hasVersionID>
    </owl:NamedIndividual>
    


    <!-- http://purl.org/htp#HiTOP-T01A5i -->

    <owl:NamedIndividual rdf:about="http://purl.org/htp#HiTOP-T01A5i">
        <rdf:type rdf:resource="http://purl.org/htp#HiTOP-O002sP"/>
        <hasVersionID>1.0</hasVersionID>
    </owl:NamedIndividual>
    


    <!-- http://purl.org/htp#HiTOP-T01BfQ -->

    <owl:NamedIndividual rdf:about="http://purl.org/htp#HiTOP-T01BfQ">
        <rdf:type rdf:resource="http://purl.org/htp#HiTOP-O002sP"/>
        <hasVersionID>1.0</hasVersionID>
    </owl:NamedIndividual>
    


    <!-- http://purl.org/htp#HiTOP-T01C1W -->

    <owl:NamedIndividual rdf:about="http://purl.org/htp#HiTOP-T01C1W">
        <rdf:type rdf:resource="http://purl.org/htp#HiTOP-O002sP"/>
        <hasVersionID>1.0</hasVersionID>
    </owl:NamedIndividual>
    


    <!-- http://purl.org/htp#HiTOP-T01Neb -->

    <owl:NamedIndividual rdf:about="http://purl.org/htp#HiTOP-T01Neb">
        <rdf:type rdf:resource="http://purl.org/htp#HiTOP-O002sP"/>
        <hasVersionID>1.0</hasVersionID>
    </owl:NamedIndividual>
    


    <!-- http://purl.org/htp#HiTOP-T01OY2 -->

    <owl:NamedIndividual rdf:about="http://purl.org/htp#HiTOP-T01OY2">
        <rdf:type rdf:resource="http://purl.org/htp#HiTOP-O002sP"/>
        <hasVersionID>1.0</hasVersionID>
    </owl:NamedIndividual>
    


    <!-- http://purl.org/htp#HiTOP-T01PMW -->

    <owl:NamedIndividual rdf:about="http://purl.org/htp#HiTOP-T01PMW">
        <rdf:type rdf:resource="http://purl.org/htp#HiTOP-O002sP"/>
        <hasVersionID>1.0</hasVersionID>
    </owl:NamedIndividual>
    


    <!-- http://purl.org/htp#HiTOP-T01QNN -->

    <owl:NamedIndividual rdf:about="http://purl.org/htp#HiTOP-T01QNN">
        <rdf:type rdf:resource="http://purl.org/htp#HiTOP-O002sP"/>
        <hasVersionID>1.0</hasVersionID>
    </owl:NamedIndividual>
    


    <!-- http://purl.org/htp#HiTOP-T01RYG -->

    <owl:NamedIndividual rdf:about="http://purl.org/htp#HiTOP-T01RYG">
        <rdf:type rdf:resource="http://purl.org/htp#HiTOP-O002sP"/>
        <hasVersionID>1.0</hasVersionID>
    </owl:NamedIndividual>
    


    <!-- http://purl.org/htp#HiTOP-T01SYW -->

    <owl:NamedIndividual rdf:about="http://purl.org/htp#HiTOP-T01SYW">
        <rdf:type rdf:resource="http://purl.org/htp#HiTOP-O002sP"/>
        <hasVersionID>1.0</hasVersionID>
    </owl:NamedIndividual>
    


    <!-- http://purl.org/htp#HiTOP-T01T3u -->

    <owl:NamedIndividual rdf:about="http://purl.org/htp#HiTOP-T01T3u">
        <rdf:type rdf:resource="http://purl.org/htp#HiTOP-O002sP"/>
        <hasVersionID>1.0</hasVersionID>
    </owl:NamedIndividual>
    


    <!-- http://purl.org/htp#HiTOP-T01UGN -->

    <owl:NamedIndividual rdf:about="http://purl.org/htp#HiTOP-T01UGN">
        <rdf:type rdf:resource="http://purl.org/htp#HiTOP-O002sP"/>
        <hasVersionID>1.0</hasVersionID>
    </owl:NamedIndividual>
    


    <!-- http://purl.org/htp#HiTOP-T01VXq -->

    <owl:NamedIndividual rdf:about="http://purl.org/htp#HiTOP-T01VXq">
        <rdf:type rdf:resource="http://purl.org/htp#HiTOP-O002sP"/>
        <hasVersionID>1.0</hasVersionID>
    </owl:NamedIndividual>
    


    <!-- http://purl.org/htp#HiTOP-T01W1E -->

    <owl:NamedIndividual rdf:about="http://purl.org/htp#HiTOP-T01W1E">
        <rdf:type rdf:resource="http://purl.org/htp#HiTOP-O002sP"/>
        <hasVersionID>1.0</hasVersionID>
    </owl:NamedIndividual>
    


    <!-- http://purl.org/htp#HiTOP-T01XQi -->

    <owl:NamedIndividual rdf:about="http://purl.org/htp#HiTOP-T01XQi">
        <rdf:type rdf:resource="http://purl.org/htp#HiTOP-O002sP"/>
        <hasVersionID>1.0</hasVersionID>
    </owl:NamedIndividual>
    


    <!-- http://purl.org/htp#HiTOP-T01Y7w -->

    <owl:NamedIndividual rdf:about="http://purl.org/htp#HiTOP-T01Y7w">
        <rdf:type rdf:resource="http://purl.org/htp#HiTOP-O002sP"/>
        <hasVersionID>1.0</hasVersionID>
    </owl:NamedIndividual>
    


    <!-- http://purl.org/htp#HiTOP-T01Ziz -->

    <owl:NamedIndividual rdf:about="http://purl.org/htp#HiTOP-T01Ziz">
        <rdf:type rdf:resource="http://purl.org/htp#HiTOP-O002sP"/>
        <hasVersionID>1.0</hasVersionID>
    </owl:NamedIndividual>
    


    <!-- http://purl.org/htp#HiTOP-T01a7u -->

    <owl:NamedIndividual rdf:about="http://purl.org/htp#HiTOP-T01a7u">
        <rdf:type rdf:resource="http://purl.org/htp#HiTOP-O002sP"/>
        <hasVersionID>1.0</hasVersionID>
    </owl:NamedIndividual>
    


    <!-- http://purl.org/htp#HiTOP-T01bz7 -->

    <owl:NamedIndividual rdf:about="http://purl.org/htp#HiTOP-T01bz7">
        <rdf:type rdf:resource="http://purl.org/htp#HiTOP-O002sP"/>
        <hasVersionID>1.0</hasVersionID>
    </owl:NamedIndividual>
    


    <!-- http://purl.org/htp#HiTOP-T01cX5 -->

    <owl:NamedIndividual rdf:about="http://purl.org/htp#HiTOP-T01cX5">
        <rdf:type rdf:resource="http://purl.org/htp#HiTOP-O002sP"/>
        <hasVersionID>1.0</hasVersionID>
    </owl:NamedIndividual>
    


    <!-- http://purl.org/htp#HiTOP-T01d9I -->

    <owl:NamedIndividual rdf:about="http://purl.org/htp#HiTOP-T01d9I">
        <rdf:type rdf:resource="http://purl.org/htp#HiTOP-O002sP"/>
        <hasVersionID>1.0</hasVersionID>
    </owl:NamedIndividual>
    


    <!-- http://purl.org/htp#HiTOP-T01eG6 -->

    <owl:NamedIndividual rdf:about="http://purl.org/htp#HiTOP-T01eG6">
        <rdf:type rdf:resource="http://purl.org/htp#HiTOP-O002sP"/>
        <hasVersionID>1.0</hasVersionID>
    </owl:NamedIndividual>
    


    <!-- http://purl.org/htp#HiTOP-T01fc8 -->

    <owl:NamedIndividual rdf:about="http://purl.org/htp#HiTOP-T01fc8">
        <rdf:type rdf:resource="http://purl.org/htp#HiTOP-O002sP"/>
        <hasVersionID>1.0</hasVersionID>
    </owl:NamedIndividual>
    


    <!-- http://purl.org/htp#HiTOP-T01gKP -->

    <owl:NamedIndividual rdf:about="http://purl.org/htp#HiTOP-T01gKP">
        <rdf:type rdf:resource="http://purl.org/htp#HiTOP-O002sP"/>
        <hasVersionID>1.0</hasVersionID>
    </owl:NamedIndividual>
    


    <!-- http://purl.org/htp#VersionHistory -->

    <owl:NamedIndividual rdf:about="http://purl.org/htp#VersionHistory">
        <rdfs:comment xml:lang="en">This resource documents the version history of the HiTOP model, detailing the changes made in each version.</rdfs:comment>
        <rdfs:label xml:lang="en">Version History</rdfs:label>
    </owl:NamedIndividual>
    


    <!-- http://purl.org/htp#Version_1_0 -->

    <owl:NamedIndividual rdf:about="http://purl.org/htp#Version_1_0">
        <partOfVersionHistory rdf:resource="http://purl.org/htp#VersionHistory"/>
        <hasVersionID>1.0</hasVersionID>
        <versionDescription>Initial release of the HiTOP model with basic structure and categories for mental health classification.</versionDescription>
    </owl:NamedIndividual>
    


    <!-- http://purl.org/htp#versionDescription -->

    <owl:NamedIndividual rdf:about="http://purl.org/htp#versionDescription">
        <rdf:type rdf:resource="http://www.w3.org/1999/02/22-rdf-syntax-ns#DatatypeProperty"/>
    </owl:NamedIndividual>
    


    <!-- 
    ///////////////////////////////////////////////////////////////////////////////////////
    //
    // Annotations
    //
    ///////////////////////////////////////////////////////////////////////////////////////
     -->

    <rdf:Description rdf:about="http://purl.org/htp#HiTOP-C001qy">
        <rdfs:comment xml:lang="en">A component related to conversion disorders where psychological distress is expressed as physical symptoms.</rdfs:comment>
        <rdfs:label xml:lang="en">Conversion</rdfs:label>
    </rdf:Description>
    <rdf:Description rdf:about="http://purl.org/htp#HiTOP-C00217">
        <rdfs:comment xml:lang="en">A component involving the expression of psychological distress through physical symptoms.</rdfs:comment>
        <rdfs:label xml:lang="en">Somatization</rdfs:label>
    </rdf:Description>
    <rdf:Description rdf:about="http://purl.org/htp#HiTOP-C0033z">
        <rdfs:comment xml:lang="en">A component related to general discomfort or unease.</rdfs:comment>
        <rdfs:label xml:lang="en">Malaise</rdfs:label>
    </rdf:Description>
    <rdf:Description rdf:about="http://purl.org/htp#HiTOP-C00416">
        <rdfs:comment xml:lang="en">A component related to headaches or other types of head pain.</rdfs:comment>
        <rdfs:label xml:lang="en">Head Pain</rdfs:label>
    </rdf:Description>
    <rdf:Description rdf:about="http://purl.org/htp#HiTOP-C005Sv">
        <rdfs:comment xml:lang="en">A component related to gastrointestinal symptoms and disorders.</rdfs:comment>
        <rdfs:label xml:lang="en">Gastrointestinal</rdfs:label>
    </rdf:Description>
    <rdf:Description rdf:about="http://purl.org/htp#HiTOP-C006MD">
        <rdfs:comment xml:lang="en">A component related to cognitive symptoms and dysfunctions.</rdfs:comment>
        <rdfs:label xml:lang="en">Cognitive</rdfs:label>
    </rdf:Description>
    <rdf:Description rdf:about="http://purl.org/htp#HiTOP-C00JTU">
        <rdfs:comment xml:lang="en">Anxiety experienced in social interactions and group settings.</rdfs:comment>
        <rdfs:label xml:lang="en">Interactive anxiety</rdfs:label>
    </rdf:Description>
    <rdf:Description rdf:about="http://purl.org/htp#HiTOP-C00KL0">
        <rdfs:comment xml:lang="en">Anxiety related to performing tasks or activities, often in public or under observation.</rdfs:comment>
        <rdfs:label xml:lang="en">Performance anxiety</rdfs:label>
    </rdf:Description>
    <rdf:Description rdf:about="http://purl.org/htp#HiTOP-C00LqY">
        <rdfs:comment xml:lang="en">Fear or anxiety associated with being in public spaces.</rdfs:comment>
        <rdfs:label xml:lang="en">Public places</rdfs:label>
    </rdf:Description>
    <rdf:Description rdf:about="http://purl.org/htp#HiTOP-C00Mpl">
        <rdfs:comment xml:lang="en">Fear or anxiety related to confined or small spaces.</rdfs:comment>
        <rdfs:label xml:lang="en">Enclosed spaces</rdfs:label>
    </rdf:Description>
    <rdf:Description rdf:about="http://purl.org/htp#HiTOP-C00N4I">
        <rdfs:comment xml:lang="en">Fear or anxiety related to animals.</rdfs:comment>
        <rdfs:label xml:lang="en">Animal phobia</rdfs:label>
    </rdf:Description>
    <rdf:Description rdf:about="http://purl.org/htp#HiTOP-C00OuR">
        <rdfs:comment xml:lang="en">Fear or anxiety related to specific situations or environments.</rdfs:comment>
        <rdfs:label xml:lang="en">Situational phobia</rdfs:label>
    </rdf:Description>
    <rdf:Description rdf:about="http://purl.org/htp#HiTOP-C00Pjp">
        <rdfs:comment xml:lang="en">Fear or anxiety related to blood, injections, or injuries.</rdfs:comment>
        <rdfs:label xml:lang="en">Blood-injection-injury</rdfs:label>
    </rdf:Description>
    <rdf:Description rdf:about="http://purl.org/htp#HiTOP-C00Q1t">
        <rdfs:comment xml:lang="en">Panic attacks characterized by physiological symptoms such as rapid heartbeat and sweating.</rdfs:comment>
        <rdfs:label xml:lang="en">Physiological panic</rdfs:label>
    </rdf:Description>
    <rdf:Description rdf:about="http://purl.org/htp#HiTOP-C00RGy">
        <rdfs:comment xml:lang="en">A component of psychological panic is an intense, overwhelming fear that triggers physical symptoms and a sense of losing control.</rdfs:comment>
        <rdfs:label xml:lang="en">Psychological panic</rdfs:label>
    </rdf:Description>
    <rdf:Description rdf:about="http://purl.org/htp#HiTOP-C00S9m">
        <rdfs:comment xml:lang="en">Compulsive behaviors related to cleaning or hygiene.</rdfs:comment>
        <rdfs:label xml:lang="en">Cleaning</rdfs:label>
    </rdf:Description>
    <rdf:Description rdf:about="http://purl.org/htp#HiTOP-C00TgL">
        <rdfs:comment xml:lang="en">Compulsive rituals or behaviors performed in a specific manner.</rdfs:comment>
        <rdfs:label xml:lang="en">Rituals</rdfs:label>
    </rdf:Description>
    <rdf:Description rdf:about="http://purl.org/htp#HiTOP-C00Urw">
        <rdfs:comment xml:lang="en">Compulsive checking behaviors, such as repeatedly checking locks or appliances.</rdfs:comment>
        <rdfs:label xml:lang="en">Checking</rdfs:label>
    </rdf:Description>
    <rdf:Description rdf:about="http://purl.org/htp#HiTOP-C00VHv">
        <rdfs:comment xml:lang="en">A state of generalized unhappiness or dissatisfaction.</rdfs:comment>
        <rdfs:label xml:lang="en">Dysphoria</rdfs:label>
    </rdf:Description>
    <rdf:Description rdf:about="http://purl.org/htp#HiTOP-C00WJc">
        <rdfs:comment xml:lang="en">A state of physical or mental weariness and lack of energy.</rdfs:comment>
        <rdfs:label xml:lang="en">Lassitude</rdfs:label>
    </rdf:Description>
    <rdf:Description rdf:about="http://purl.org/htp#HiTOP-C00XyI">
        <rdfs:comment xml:lang="en">A trait characterized by the loss of interest or pleasure in activities that are usually enjoyable.</rdfs:comment>
        <rdfs:label xml:lang="en">Anhedonia</rdfs:label>
    </rdf:Description>
    <rdf:Description rdf:about="http://purl.org/htp#HiTOP-C00Y8j">
        <rdfs:comment xml:lang="en">Difficulty falling asleep or staying asleep, or waking up too early and not being able to go back to sleep.</rdfs:comment>
        <rdfs:label xml:lang="en">Insomnia</rdfs:label>
    </rdf:Description>
    <rdf:Description rdf:about="http://purl.org/htp#HiTOP-C00ZyP">
        <rdfs:comment xml:lang="en">The presence of thoughts or behaviors related to suicide.</rdfs:comment>
        <rdfs:label xml:lang="en">Suicidality</rdfs:label>
    </rdf:Description>
    <rdf:Description rdf:about="http://purl.org/htp#HiTOP-C00aMF">
        <rdfs:comment xml:lang="en">State of being overly excited or disturbed, often resulting in restlessness or erratic behavior.</rdfs:comment>
        <rdfs:label xml:lang="en">Agitation</rdfs:label>
    </rdf:Description>
    <rdf:Description rdf:about="http://purl.org/htp#HiTOP-C00bEx">
        <rdfs:comment xml:lang="en">
            Slowed cognitive and physical processes, including thinking, speaking, and moving. 
            As the term 'retardation' is considered sensitive and potentially stigmatizing, the expression 
            'psychomotor retardation' is more commonly used in current clinical contexts. 
            This definition adheres to the classical vocabulary used in the HiTOP working model. 
        </rdfs:comment>
        <rdfs:label xml:lang="en">Retardation</rdfs:label>
    </rdf:Description>
    <rdf:Description rdf:about="http://purl.org/htp#HiTOP-C00cSn">
        <rdfs:comment xml:lang="en">Reduction or loss of desire to eat, which can lead to weight loss.</rdfs:comment>
        <rdfs:label xml:lang="en">Appetite loss</rdfs:label>
    </rdf:Description>
    <rdf:Description rdf:about="http://purl.org/htp#HiTOP-C00dc1">
        <rdfs:comment xml:lang="en">Increased desire to eat, which can lead to weight gain.</rdfs:comment>
        <rdfs:label xml:lang="en">Appetite gain</rdfs:label>
    </rdf:Description>
    <rdf:Description rdf:about="http://purl.org/htp#HiTOP-C00eL">
        <rdfs:comment xml:lang="en">A positive state of mental and physical health, encompassing feelings of happiness and contentment.</rdfs:comment>
        <rdfs:label xml:lang="en">(low) Wellbeing</rdfs:label>
    </rdf:Description>
    <rdf:Description rdf:about="http://purl.org/htp#HiTOP-C00fKQ">
        <rdfs:comment xml:lang="en">A component of generalized anxiety disorder symptoms is excessive, persistent worry that interferes with daily life and is often accompanied by physical symptoms like restlessness and fatigue.</rdfs:comment>
        <rdfs:label xml:lang="en">Generalized anxiety disorder symptoms</rdfs:label>
    </rdf:Description>
    <rdf:Description rdf:about="http://purl.org/htp#HiTOP-C00gvD">
        <rdfs:comment xml:lang="en">Re-living traumatic events through flashbacks, intrusive memories, or nightmares.</rdfs:comment>
        <rdfs:label xml:lang="en">Re-experiencing</rdfs:label>
    </rdf:Description>
    <rdf:Description rdf:about="http://purl.org/htp#HiTOP-C00hPJ">
        <rdfs:comment xml:lang="en">Efforts to avoid reminders or situations that are associated with traumatic experiences or stress.</rdfs:comment>
        <rdfs:label xml:lang="en">Avoidance</rdfs:label>
    </rdf:Description>
    <rdf:Description rdf:about="http://purl.org/htp#HiTOP-C00iAh">
        <rdfs:comment xml:lang="en">Increased physiological arousal, including symptoms such as hypervigilance, irritability, and difficulty sleeping.</rdfs:comment>
        <rdfs:label xml:lang="en">Hyperarousal</rdfs:label>
    </rdf:Description>
    <rdf:Description rdf:about="http://purl.org/htp#HiTOP-C00jw5">
        <rdfs:comment xml:lang="en">Emotional numbness or detachment from feelings as a response to overwhelming stress or trauma.</rdfs:comment>
        <rdfs:label xml:lang="en">Numbing</rdfs:label>
    </rdf:Description>
    <rdf:Description rdf:about="http://purl.org/htp#HiTOP-C00kEN">
        <rdfs:comment xml:lang="en">A mental process used to cope with stress or trauma, leading to a sense of detachment from one&apos;s surroundings or self.</rdfs:comment>
        <rdfs:label xml:lang="en">Dissociation</rdfs:label>
    </rdf:Description>
    <rdf:Description rdf:about="http://purl.org/htp#HiTOP-C00l5y">
        <rdfs:comment xml:lang="en">State of being easily annoyed or angered, often with a low tolerance for frustration.</rdfs:comment>
        <rdfs:label xml:lang="en">Irritability</rdfs:label>
    </rdf:Description>
    <rdf:Description rdf:about="http://purl.org/htp#HiTOP-C00mpe">
        <rdfs:comment xml:lang="en">Recurrent and persistent intrusive thoughts that cause significant distress, without accompanying compulsive behaviors.</rdfs:comment>
        <rdfs:label xml:lang="en">Pure obsessions</rdfs:label>
    </rdf:Description>
    <rdf:Description rdf:about="http://purl.org/htp#HiTOP-C00nyb">
        <rdfs:comment xml:lang="en">A state of heightened mood and increased energy, often associated with mania or hypomania.</rdfs:comment>
        <rdfs:label xml:lang="en">Euphoric activation</rdfs:label>
    </rdf:Description>
    <rdf:Description rdf:about="http://purl.org/htp#HiTOP-C00oKM">
        <rdfs:comment xml:lang="en">Increased cognitive activity, often characterized by racing thoughts and distractibility.</rdfs:comment>
        <rdfs:label xml:lang="en">Hyperactive cognition</rdfs:label>
    </rdf:Description>
    <rdf:Description rdf:about="http://purl.org/htp#HiTOP-C00pnZ">
        <rdfs:comment xml:lang="en">Excessive self-confidence leading to risky or impulsive behavior, often seen in manic episodes.</rdfs:comment>
        <rdfs:label xml:lang="en">Reckless overconfidence</rdfs:label>
    </rdf:Description>
    <rdf:Description rdf:about="http://purl.org/htp#HiTOP-C00qSD">
        <rdfs:comment xml:lang="en">A component characterized by symptoms of psychosis.</rdfs:comment>
        <rdfs:label xml:lang="en">Psychotic</rdfs:label>
    </rdf:Description>
    <rdf:Description rdf:about="http://purl.org/htp#HiTOP-C00rnS">
        <rdfs:comment xml:lang="en">A component characterized by disorganized thinking and behavior.</rdfs:comment>
        <rdfs:label xml:lang="en">Disorganized</rdfs:label>
    </rdf:Description>
    <rdf:Description rdf:about="http://purl.org/htp#HiTOP-C00sWr">
        <rdfs:comment xml:lang="en">A component characterized by a lack of emotional expression.</rdfs:comment>
        <rdfs:label xml:lang="en">Inexpressivity</rdfs:label>
    </rdf:Description>
    <rdf:Description rdf:about="http://purl.org/htp#HiTOP-C00tUQ">
        <rdfs:comment xml:lang="en">A component characterized by a lack of motivation to initiate and sustain purposeful activities.</rdfs:comment>
        <rdfs:label xml:lang="en">Avolition</rdfs:label>
    </rdf:Description>
    <rdf:Description rdf:about="http://purl.org/htp#HiTOP-C01DAb">
        <rdfs:comment xml:lang="en">The consumption of alcoholic beverages, which may lead to problematic use.</rdfs:comment>
        <rdfs:label xml:lang="en">Alcohol use</rdfs:label>
    </rdf:Description>
    <rdf:Description rdf:about="http://purl.org/htp#HiTOP-C01Elz">
        <rdfs:comment xml:lang="en">Issues related to the use of alcohol, including dependence and abuse.</rdfs:comment>
        <rdfs:label xml:lang="en">Alcohol problems</rdfs:label>
    </rdf:Description>
    <rdf:Description rdf:about="http://purl.org/htp#HiTOP-C01FDy">
        <rdfs:comment xml:lang="en">The consumption of marijuana, which may lead to problematic use.</rdfs:comment>
        <rdfs:label xml:lang="en">Marijuana use</rdfs:label>
    </rdf:Description>
    <rdf:Description rdf:about="http://purl.org/htp#HiTOP-C01GEY">
        <rdfs:comment xml:lang="en">Issues related to the use of marijuana, including dependence and abuse.</rdfs:comment>
        <rdfs:label xml:lang="en">Marijuana problems</rdfs:label>
    </rdf:Description>
    <rdf:Description rdf:about="http://purl.org/htp#HiTOP-C01HGq">
        <rdfs:comment xml:lang="en">The consumption of illicit or prescription drugs, which may lead to problematic use.</rdfs:comment>
        <rdfs:label xml:lang="en">Drug use</rdfs:label>
    </rdf:Description>
    <rdf:Description rdf:about="http://purl.org/htp#HiTOP-C01Ip4">
        <rdfs:comment xml:lang="en">Issues related to the use of drugs, including dependence and abuse.</rdfs:comment>
        <rdfs:label xml:lang="en">Drug problems</rdfs:label>
    </rdf:Description>
    <rdf:Description rdf:about="http://purl.org/htp#HiTOP-C01JH8">
        <rdfs:comment xml:lang="en">Aggression involving physical acts of violence towards others.</rdfs:comment>
        <rdfs:label xml:lang="en">Physical aggression</rdfs:label>
    </rdf:Description>
    <rdf:Description rdf:about="http://purl.org/htp#HiTOP-C01KXo">
        <rdfs:comment xml:lang="en">Aggression that results in damage to property or the environment.</rdfs:comment>
        <rdfs:label xml:lang="en">Destructive aggression</rdfs:label>
    </rdf:Description>
    <rdf:Description rdf:about="http://purl.org/htp#HiTOP-C01LSp">
        <rdfs:comment xml:lang="en">Aggression that harms others through manipulation of social relationships.</rdfs:comment>
        <rdfs:label xml:lang="en">Relational aggression</rdfs:label>
    </rdf:Description>
    <rdf:Description rdf:about="http://purl.org/htp#HiTOP-C01MjB">
        <rdfs:comment xml:lang="en">Deceptive behavior intended to secure unfair or unlawful gain.</rdfs:comment>
        <rdfs:label xml:lang="en">Fraud</rdfs:label>
    </rdf:Description>
    <rdf:Description rdf:about="http://purl.org/htp#HiTOP-T007eM">
        <rdfs:comment xml:lang="en">A trait characterized by a tendency to experience anxiety or nervousness.</rdfs:comment>
        <rdfs:label xml:lang="en">Anxiousness</rdfs:label>
    </rdf:Description>
    <rdf:Description rdf:about="http://purl.org/htp#HiTOP-T008mD">
        <rdfs:comment xml:lang="en">A trait characterized by rapid and intense emotional changes.</rdfs:comment>
        <rdfs:label xml:lang="en">Emotional lability</rdfs:label>
    </rdf:Description>
    <rdf:Description rdf:about="http://purl.org/htp#HiTOP-T0094I">
        <rdfs:comment xml:lang="en">A trait characterized by a tendency toward aggression or antagonism.</rdfs:comment>
        <rdfs:label xml:lang="en">Hostility</rdfs:label>
    </rdf:Description>
    <rdf:Description rdf:about="http://purl.org/htp#HiTOP-T00AZ">
        <rdfs:comment xml:lang="en">A trait characterized by the repetition of a particular response despite the absence or cessation of a stimulus.</rdfs:comment>
        <rdfs:label xml:lang="en">Perseveration</rdfs:label>
    </rdf:Description>
    <rdf:Description rdf:about="http://purl.org/htp#HiTOP-T00BXK">
        <rdfs:comment xml:lang="en">A trait characterized by limited or constricted emotional expression.</rdfs:comment>
        <rdfs:label xml:lang="en">(low) Restricted affectivity</rdfs:label>
    </rdf:Description>
    <rdf:Description rdf:about="http://purl.org/htp#HiTOP-T00Cgy">
        <rdfs:comment xml:lang="en">A trait characterized by anxiety and insecurity in response to separation from significant others.</rdfs:comment>
        <rdfs:label xml:lang="en">Separation insecurity</rdfs:label>
    </rdf:Description>
    <rdf:Description rdf:about="http://purl.org/htp#HiTOP-T00D42">
        <rdfs:comment xml:lang="en">A trait characterized by a tendency to submit to others and avoid asserting oneself.</rdfs:comment>
        <rdfs:label xml:lang="en">Submissiveness</rdfs:label>
    </rdf:Description>
    <rdf:Description rdf:about="http://purl.org/htp#HiTOP-T00Eht">
        <rdfs:comment xml:lang="en">A trait characterized by difficulties in forming or maintaining a stable sense of self.</rdfs:comment>
        <rdfs:label xml:lang="en">Identity problems</rdfs:label>
    </rdf:Description>
    <rdf:Description rdf:about="http://purl.org/htp#HiTOP-T00Fe0">
        <rdfs:comment xml:lang="en">A trait of negative relationships is that they contribute to stress, conflict, or emotional harm, often undermining well-being and personal growth.</rdfs:comment>
        <rdfs:label xml:lang="en">Negative relationships</rdfs:label>
    </rdf:Description>
    <rdf:Description rdf:about="http://purl.org/htp#HiTOP-T00G3d">
        <rdfs:comment xml:lang="en">A trait characterized by a lack of resilience and a tendency to be easily hurt or affected by stress.</rdfs:comment>
        <rdfs:label xml:lang="en">Fragility</rdfs:label>
    </rdf:Description>
    <rdf:Description rdf:about="http://purl.org/htp#HiTOP-T00HCy">
        <rdfs:comment xml:lang="en">A trait characterized by a lack of skill or competence.</rdfs:comment>
        <rdfs:label xml:lang="en">Ineptitude</rdfs:label>
    </rdf:Description>
    <rdf:Description rdf:about="http://purl.org/htp#HiTOP-T00IAT">
        <rdfs:comment xml:lang="en">A trait characterized by a perception of being immune to harm or negative effects.</rdfs:comment>
        <rdfs:label xml:lang="en">(low) Invulnerability</rdfs:label>
    </rdf:Description>
    <rdf:Description rdf:about="http://purl.org/htp#HiTOP-T00ua9">
        <rdfs:comment xml:lang="en">A trait characterized by unconventional or peculiar behavior.</rdfs:comment>
        <rdfs:label xml:lang="en">Eccentricity</rdfs:label>
    </rdf:Description>
    <rdf:Description rdf:about="http://purl.org/htp#HiTOP-T00vjR">
        <rdfs:comment xml:lang="en">A trait characterized by disturbances in cognition and perception.</rdfs:comment>
        <rdfs:label xml:lang="en">Cognitive perceptual dysregulation</rdfs:label>
    </rdf:Description>
    <rdf:Description rdf:about="http://purl.org/htp#HiTOP-T00wk6">
        <rdfs:comment xml:lang="en">A trait characterized by the presence of atypical beliefs and experiences.</rdfs:comment>
        <rdfs:label xml:lang="en">Unusual beliefs and experiences</rdfs:label>
    </rdf:Description>
    <rdf:Description rdf:about="http://purl.org/htp#HiTOP-T00xLn">
        <rdfs:comment xml:lang="en">A trait characterized by a tendency to engage in vivid and complex fantasies.</rdfs:comment>
        <rdfs:label xml:lang="en">Fantasy proneness</rdfs:label>
    </rdf:Description>
    <rdf:Description rdf:about="http://purl.org/htp#HiTOP-T00yfU">
        <rdfs:comment xml:lang="en">A trait characterized by feelings of sadness and hopelessness.</rdfs:comment>
        <rdfs:label xml:lang="en">Depressivity</rdfs:label>
    </rdf:Description>
    <rdf:Description rdf:about="http://purl.org/htp#HiTOP-T00zDk">
        <rdfs:comment xml:lang="en">A trait characterized by a tendency to avoid close relationships and emotional intimacy.</rdfs:comment>
        <rdfs:label xml:lang="en">Intimacy avoidance</rdfs:label>
    </rdf:Description>
    <rdf:Description rdf:about="http://purl.org/htp#HiTOP-T010c6">
        <rdfs:comment xml:lang="en">A trait characterized by a tendency to be distrustful and suspicious of others.</rdfs:comment>
        <rdfs:label xml:lang="en">Suspiciousness</rdfs:label>
    </rdf:Description>
    <rdf:Description rdf:about="http://purl.org/htp#HiTOP-T011K6">
        <rdfs:comment xml:lang="en">A trait characterized by a tendency to retreat from social interactions and avoid engagement with others.</rdfs:comment>
        <rdfs:label xml:lang="en">Withdrawal</rdfs:label>
    </rdf:Description>
    <rdf:Description rdf:about="http://purl.org/htp#HiTOP-T012QL">
        <rdfs:comment xml:lang="en">A trait characterized by a lack of initiative or assertiveness in social interactions.</rdfs:comment>
        <rdfs:label xml:lang="en">Interpersonal passivity</rdfs:label>
    </rdf:Description>
    <rdf:Description rdf:about="http://purl.org/htp#HiTOP-T013F1">
        <rdfs:comment xml:lang="en">A trait characterized by a lack of interest in forming or maintaining social bonds.</rdfs:comment>
        <rdfs:label xml:lang="en">Disaffiliativeness</rdfs:label>
    </rdf:Description>
    <rdf:Description rdf:about="http://purl.org/htp#HiTOP-T014BA">
        <rdfs:comment xml:lang="en">A trait characterized by a strong desire to attract and hold the attention of others.</rdfs:comment>
        <rdfs:label xml:lang="en">(low) Attention seeking</rdfs:label>
    </rdf:Description>
    <rdf:Description rdf:about="http://purl.org/htp#HiTOP-T015o8">
        <rdfs:comment xml:lang="en">A trait characterized by difficulty in controlling impulsive behaviors, often leading to negative consequences.</rdfs:comment>
        <rdfs:label xml:lang="en">Problematic impulsivity</rdfs:label>
    </rdf:Description>
    <rdf:Description rdf:about="http://purl.org/htp#HiTOP-T016k0">
        <rdfs:comment xml:lang="en">A trait characterized by a lack of regard for the consequences of one&apos;s actions, often leading to reckless behavior.</rdfs:comment>
        <rdfs:label xml:lang="en">Irresponsibility</rdfs:label>
    </rdf:Description>
    <rdf:Description rdf:about="http://purl.org/htp#HiTOP-T0177S">
        <rdfs:comment xml:lang="en">A trait characterized by a tendency to steal or engage in dishonest acquisition of property.</rdfs:comment>
        <rdfs:label xml:lang="en">Theft</rdfs:label>
    </rdf:Description>
    <rdf:Description rdf:about="http://purl.org/htp#HiTOP-T018ir">
        <rdfs:comment xml:lang="en">A trait characterized by an inability to maintain focus, leading to frequent shifts in attention.</rdfs:comment>
        <rdfs:label xml:lang="en">Distractibility</rdfs:label>
    </rdf:Description>
    <rdf:Description rdf:about="http://purl.org/htp#HiTOP-T019Cj">
        <rdfs:comment xml:lang="en">A trait characterized by engaging in behaviors that involve significant risk, often without regard for potential negative outcomes.</rdfs:comment>
        <rdfs:label xml:lang="en">Risk taking</rdfs:label>
    </rdf:Description>
    <rdf:Description rdf:about="http://purl.org/htp#HiTOP-T01A5i">
        <rdfs:comment xml:lang="en">A trait characterized by an excessive and inflexible striving for perfection and high standards, often leading to self-criticism and stress.</rdfs:comment>
        <rdfs:label xml:lang="en">(low) Rigid perfectionism</rdfs:label>
    </rdf:Description>
    <rdf:Description rdf:about="http://purl.org/htp#HiTOP-T01BfQ">
        <rdfs:comment xml:lang="en">A trait characterized by excessive and repetitive thinking about potential decisions and their outcomes, often leading to indecision and stress.</rdfs:comment>
        <rdfs:label xml:lang="en">(low) Ruminative deliberation</rdfs:label>
    </rdf:Description>
    <rdf:Description rdf:about="http://purl.org/htp#HiTOP-T01C1W">
        <rdfs:comment xml:lang="en">A trait characterized by an excessive and compulsive commitment to work, often at the expense of personal well-being and relationships.</rdfs:comment>
        <rdfs:label xml:lang="en">(low) Workaholism</rdfs:label>
    </rdf:Description>
    <rdf:Description rdf:about="http://purl.org/htp#HiTOP-T01Neb">
        <rdfs:comment xml:lang="en">A trait characterized by a lack of patience and a tendency to act impulsively in urgent situations.</rdfs:comment>
        <rdfs:label xml:lang="en">Impatient urgency</rdfs:label>
    </rdf:Description>
    <rdf:Description rdf:about="http://purl.org/htp#HiTOP-T01OY2">
        <rdfs:comment xml:lang="en">A trait indicating poor ability to plan and execute tasks effectively.</rdfs:comment>
        <rdfs:label xml:lang="en">(low) Planful control</rdfs:label>
    </rdf:Description>
    <rdf:Description rdf:about="http://purl.org/htp#HiTOP-T01PMW">
        <rdfs:comment xml:lang="en">A trait characterized by a lack of reliability and consistency in fulfilling obligations.</rdfs:comment>
        <rdfs:label xml:lang="en">(low) Dependability</rdfs:label>
    </rdf:Description>
    <rdf:Description rdf:about="http://purl.org/htp#HiTOP-T01QNN">
        <rdfs:comment xml:lang="en">A trait reflecting a sense of estrangement or detachment from others.</rdfs:comment>
        <rdfs:label xml:lang="en">Alienation</rdfs:label>
    </rdf:Description>
    <rdf:Description rdf:about="http://purl.org/htp#HiTOP-T01RYG">
        <rdfs:comment xml:lang="en">A trait indicating a tendency to experience boredom frequently and easily.</rdfs:comment>
        <rdfs:label xml:lang="en">Boredom proneness</rdfs:label>
    </rdf:Description>
    <rdf:Description rdf:about="http://purl.org/htp#HiTOP-T01SYW">
        <rdfs:comment xml:lang="en">A trait characterized by a tendency to attribute failures or problems to external factors rather than internal ones.</rdfs:comment>
        <rdfs:label xml:lang="en">Blame externalization</rdfs:label>
    </rdf:Description>
    <rdf:Description rdf:about="http://purl.org/htp#HiTOP-T01T3u">
        <rdfs:comment xml:lang="en">A trait marked by a tendency to be deceitful or untruthful.</rdfs:comment>
        <rdfs:label xml:lang="en">(low) Honesty</rdfs:label>
    </rdf:Description>
    <rdf:Description rdf:about="http://purl.org/htp#HiTOP-T01UGN">
        <rdfs:comment xml:lang="en">A trait characterized by resistance to authority and norms.</rdfs:comment>
        <rdfs:label xml:lang="en">Rebelliousness</rdfs:label>
    </rdf:Description>
    <rdf:Description rdf:about="http://purl.org/htp#HiTOP-T01VXq">
        <rdfs:comment xml:lang="en">A trait indicating a reduced ability to understand and share the feelings of others.</rdfs:comment>
        <rdfs:label xml:lang="en">(low) Empathy</rdfs:label>
    </rdf:Description>
    <rdf:Description rdf:about="http://purl.org/htp#HiTOP-T01W1E">
        <rdfs:comment xml:lang="en">A trait characterized by a desire for new, thrilling, or risky experiences.</rdfs:comment>
        <rdfs:label xml:lang="en">Excitement seeking</rdfs:label>
    </rdf:Description>
    <rdf:Description rdf:about="http://purl.org/htp#HiTOP-T01XQi">
        <rdfs:comment xml:lang="en">A trait of attention seeking is the constant need for validation or recognition, often leading to behavior aimed at drawing focus from others.</rdfs:comment>
        <rdfs:label xml:lang="en">Attention seeking</rdfs:label>
    </rdf:Description>
    <rdf:Description rdf:about="http://purl.org/htp#HiTOP-T01Y7w">
        <rdfs:comment xml:lang="en">A trait characterized by a lack of empathy and a tendency to be emotionally cold or indifferent to others.</rdfs:comment>
        <rdfs:label xml:lang="en">Callousness</rdfs:label>
    </rdf:Description>
    <rdf:Description rdf:about="http://purl.org/htp#HiTOP-T01Ziz">
        <rdfs:comment xml:lang="en">A trait characterized by a tendency to lie, cheat, or deceive others.</rdfs:comment>
        <rdfs:label xml:lang="en">Deceitfulness</rdfs:label>
    </rdf:Description>
    <rdf:Description rdf:about="http://purl.org/htp#HiTOP-T01a7u">
        <rdfs:comment xml:lang="en">A trait characterized by an exaggerated sense of one&apos;s own importance, abilities, or achievements.</rdfs:comment>
        <rdfs:label xml:lang="en">Grandiosity</rdfs:label>
    </rdf:Description>
    <rdf:Description rdf:about="http://purl.org/htp#HiTOP-T01bz7">
        <rdfs:comment xml:lang="en">A trait characterized by a tendency to control or influence others for personal gain, often in a devious manner.</rdfs:comment>
        <rdfs:label xml:lang="en">Manipulativeness</rdfs:label>
    </rdf:Description>
    <rdf:Description rdf:about="http://purl.org/htp#HiTOP-T01cX5">
        <rdfs:comment xml:lang="en">A trait characterized by a lack of manners or respect in social interactions.</rdfs:comment>
        <rdfs:label xml:lang="en">Rudeness</rdfs:label>
    </rdf:Description>
    <rdf:Description rdf:about="http://purl.org/htp#HiTOP-T01d9I">
        <rdfs:comment xml:lang="en">A trait characterized by an excessive focus on oneself and one&apos;s own needs and desires.</rdfs:comment>
        <rdfs:label xml:lang="en">Egocentricity</rdfs:label>
    </rdf:Description>
    <rdf:Description rdf:about="http://purl.org/htp#HiTOP-T01eG6">
        <rdfs:comment xml:lang="en">A trait characterized by a desire to control or lead others, often displaying assertiveness and power.</rdfs:comment>
        <rdfs:label xml:lang="en">Dominance</rdfs:label>
    </rdf:Description>
    <rdf:Description rdf:about="http://purl.org/htp#HiTOP-T01fc8">
        <rdfs:comment xml:lang="en">A trait characterized by behavior that seeks to attract romantic or sexual interest from others through playful or provocative means.</rdfs:comment>
        <rdfs:label xml:lang="en">Flirtatiousness</rdfs:label>
    </rdf:Description>
    <rdf:Description rdf:about="http://purl.org/htp#HiTOP-T01gKP">
        <rdfs:comment xml:lang="en">A trait characterized by a tendency to be fearful or lacking in confidence, often leading to shyness or hesitation.</rdfs:comment>
        <rdfs:label xml:lang="en">(low) Timorousness</rdfs:label>
    </rdf:Description>
    <rdf:Description rdf:about="http://purl.org/htp#versionDescription">
        <rdfs:comment xml:lang="en">A property used to describe the changes made in this version and provide an explanation of the version.</rdfs:comment>
        <rdfs:isDefinedBy rdf:resource="http://purl.org/htp#"/>
        <rdfs:label>Version Description</rdfs:label>
    </rdf:Description>
</rdf:RDF>



<!-- Generated by the OWL API (version 4.5.26.2023-07-17T20:34:13Z) https://github.com/owlcs/owlapi -->

